% !TEX root = 0-20SPAWC_SAND.tex
% DO NOT REMOVE THE ABOVE COMMENT!

\refstepcounter{section} \label{app:sand_sure}
\section*{\fref{app:sand_sure}: Derivation of SURE in \fref{eq:sure}} 

For deriving SURE as in \fref{eq:sure}, we follow the procedure in \cite[App.~A]{ghods19a}, with the following modifications: Instead of $\yhat = \hhat+\ehat$, we use $\rhat = \alpha\hhat + \dhat$. In other words, where~\cite{ghods19a} uses $\yhat\sim\CN(\hhat,\Eo\bI_B)$, we replace it by $\rhat\sim\CN(\alpha\hhat,\Do\bI_B)$. Instead of $g(\yhat) = \mu(\yhat) - \yhat$, we use $g(\rhat) = \mu(\rhat) - \rhat/\alpha$.

