\appendix
\section{A Convergence Result} 
\begin{lemma}\label{appendix_convergence}
	Consider a recurrence formula as follows:
	\begin{equation}\label{eq:sequence}
	x_{k+1} = F(x_k), \quad\forall \quad k\geq 1,
	\end{equation}
	where $F(x) = ax^2+bx+c$ and $a$, $b$, $c$ are real positive scaler numbers. Moreover, assume that $x_1 = c$.   Then, $\lim\nolimits_{k\rightarrow \infty}x_k =:x^*$ is finite if 
	\begin{subequations}
		\begin{align}
		b&<1, \quad \text{and} \label{cond1}\\
1>(b-1)^2-4ac &> 0.\label{cond2} 
\end{align}
	\end{subequations}
Furthermore,  $x^*$ is given by the smaller root of the the following quadratic equation:
$$ax^2 + (b-1)x +c = 0, \quad\text{i.e.,}$$
	\begin{equation}
	x^* = \dfrac{ -(b-1) - \sqrt{(b-1)^2-4ac}}{2a}.
	\end{equation}
	\end{lemma} 
	\begin{proof}
		First, note that the sequence \eqref{eq:sequence} contains only  real positive numbers. Thus, the equilibrium point  must also be  a real positive number. Furthermore, the equilibrium points solve the quadratic equation $F(x)-x = 0$, and we denote these equilibrium points by $x^{(1)}$ and $x^{(2)}$ with $x^{(1)}\leq x^{(2)}$.  Since $a$, $b$ and $c$ all are positive, both equilibrium points either can be positive or negative depending on the value of $b$.  To ensure the equilibrium points being positive, the minima of $F(x)-x$ must lie in the right half plane; thus, $b-1<0$, leading to the condition \eqref{cond1}. 
		
		Furthermore, we consider the derivative of $F(x)$, that is, $F'(x) := 2ax+b$.   Since $F'(x)$ is an increasing function and $F'(x) \geq 0$ $ \forall x \in [c,x^{(1)}]$, we have for $y \in [c,x^{(1)}]$:
		\begin{align*}
		 F'(y) &\leq  F'(x^{(1)})\\
		 &\leq 2ax^{(1)}+b = 2a\left(\dfrac{-(b-1) - \sqrt{(b-1)^2-4ac}}{2a} \right)  + b 
		  \leq 1 - \sqrt{(b-1)^2-4ac} .
		\end{align*}
	  Assuming  $1>(b-1)^2-4ac >0$, we have  $F'(y)  <1$, $\forall y\in [c,x^{(1)}]$.  Thus, by Banach fix-point theorem,  $F(x)$ is a contraction on $[c,x^{(1)}]$, and the fixed point is given by $x^{(1)}$.
\end{proof}
