\begin{equation}

\ket{\psi} = \alpha\ket{0} + \beta\ket{1}
\end{equation}

\begin{equation}

\ket{0} = \begin{bmatrix} 1 \\ 0 \end{bmatrix}, \quad \ket{1} = \begin{bmatrix} 0 \\ 1 \end{bmatrix}.
\end{equation}

\begin{equation}

\ket{0}\otimes\ket{0} = \begin{bmatrix} 1 \\ 0 \\ 0 \\ 0 \end{bmatrix}.
\end{equation}

\begin{equation}

\hat{U}_\textrm{QFT} = \frac{1}{\sqrt{N}} \sum_{n,m=0}^{N-1} e^{2\pi i nm/N} \ket{m}\bra{n}
\end{equation}

\begin{align}

&\textsf{\textbf{F}}_N = \nonumber\\
&\frac{1}{\sqrt{N}} \begin{bmatrix}
1 & 1 & 1 & 1 & ... & 1 \\
1 & \omega & \omega^2 & \omega^3 & ... & \omega^{N-1} \\
1 & \omega^2 & \omega^4 & \omega^6 & ... & \omega^{2(N-1)} \\
1 & \omega^3 & \omega^6 & \omega^9 & ... & \omega^{3(N-1)} \\
\vdots & \vdots & \vdots & \vdots & \ddots & \vdots \\
1 & \omega^{N-1} & \omega^{2(N-1)} & \omega^{3(N-1)} & ... & \omega^{(N-1)^2}
\end{bmatrix} \label{eq:qft-matrix}
\end{align}

\begin{equation}

\ket{\pm} = \frac{1}{\sqrt{2}} (\ket{0} \pm \ket{1}).
\end{equation}

\begin{equation}

R_N = \begin{bmatrix} 1 & 0 \\ 0 & e^{-2\pi i/N} \end{bmatrix}
\end{equation}

\begin{equation}

U \ket{\psi} = \lambda \ket{\psi},
\end{equation}

\begin{align}

\frac{1}{\sqrt{2^n}} \sum_{k=0}^{2^n-1}e^{2k\pi i\theta} \vert k \rangle.
\end{align}

\begin{equation}

\frac{1}{\sqrt{2^n}} \sum_{k=0}^{2^n-1}e^{2k\pi i\theta} \vert k \rangle \vert \psi \rangle \to \vert\tilde{\theta}\rangle \vert \psi \rangle.
\end{equation}

\begin{equation}
\label{eq:shor-f}
f(x)=a^x \text{mod}N. 
\end{equation}

\begin{gather}

\ket{0}_n \ket{2^{n_0}-1}_{n_0} \to
\frac{1}{\sqrt{2^n}} \sum_{x=0}^{2^n-1} \ket{x}_n \ket{2^{n_0}-1}_{n_0} \nonumber\\ 
\to
\frac{1}{\sqrt{2^n}} \sum_{x=0}^{2^n-1} \ket{x}_n \ket{f(x)}_{n_0}.
\end{gather}

\begin{equation}

\frac{1}{\sqrt{N}} \sum_{k=0}^{N-1} \ket{x_0+kr}_n \ket{f(x_0)}_{n_0}
\end{equation}

\begin{equation}

\mathcal{O} \ket{x} =
\begin{cases}
-\ket{x_0}, & x=x_0 \\
\ket{x}, & \textrm{otherwise.} \\
\end{cases}
\end{equation}

\begin{equation}

U_G = 2 \ket{d} \bra{d} - \mathbbm{1}
\end{equation}

\begin{equation}

r = 
\Big\lfloor \frac{\pi}{2\vartheta} \Big\rfloor 
=
\Big\lfloor \frac{\pi}{4} \sqrt{N} \Big\rfloor
\end{equation}

\begin{gather}

A = \sum_j \lambda_j\ket{u_j}\bra{u_j} \\
A^{-1} = \sum_j \lambda_j^{-1}\ket{u_j}\bra{u_j}
\end{gather}

\begin{equation}

\ket{b} = \sum_j b_j\ket{u_j}.
\end{equation}

\begin{equation}

\ket{x} = A^{-1} \ket{b} = \sum_j \lambda_j^{-1}b_j\ket{u_j}.
\end{equation}

\begin{equation}

U = e^{iAt}.
\end{equation}

\begin{equation}

\ket{b}_I \ket{0}^{\otimes N}_C = 
\sum_j \beta_j \ket{u_j}_I \ket{0}^{\otimes N}_C
\xrightarrow[]{\text{QPE}}
\sum_j \beta_j \ket{u_j}_I \ket{\tilde{\lambda}_j}_C
\end{equation}

\begin{equation}

\sum_j \beta_j \ket{u_j}_I \ket{\tilde{\lambda}_j}_C \ket{0}_S.
\end{equation}

\begin{gather}

\sum_j \beta_j \ket{u_j}_I \ket{\tilde{\lambda}_j}_C \ket{0}_S \nonumber\\
\to
\sum_j \beta_j \ket{u_j}_I \ket{\tilde{\lambda}_j}_C 
\left( 
\sqrt{1-\frac{c^2}{\lambda_j^2}}\ket{0}_S + \frac{c}{\lambda}\ket{1}_S
\right)
\end{gather}

\begin{equation}

\sum_j \beta_j \ket{u_j}_I \ket{0}^{\otimes N}_C 
\left( 
\sqrt{1-\frac{c^2}{\lambda_j^2}}\ket{0}_S + \frac{c}{\lambda}\ket{1}_S
\right).
\end{equation}

\begin{equation}

\ket{x} \approx
\sum_j \frac{\beta_j c}{\lambda_j} \ket{u_j} 
\end{equation}

\begin{equation}
\label{eq:qubo}
f(\mathbf{x}) = \sum_j Q_{jj} x_j + \sum_{j<k} Q_{jk} x_j x_k.
\end{equation}

\begin{align}

\hat{H}_\text{Ising} = A(t) \underbrace{\sum_n \hat{\sigma}^x_n}_{\hat{H}_0} + 
B(t) \underbrace{\sum_{n,m} 
\left( 
h_n \hat{\sigma}^z_n + 
J_{nm} \hat{\sigma}^z_n \hat{\sigma}^z_m 
\right)}_{\hat{H}_p}
\end{align}

\begin{equation}

U(\gamma,\beta) = \prod_k e^{-i\beta_k\hat{H}_M} e^{-i\gamma_k\hat{H}_P},
\end{equation}

\begin{equation}

\frac{d\ket{\psi(t)}}{dt} = -i\hat{H} \ket{\psi(t)}
\end{equation}

\begin{equation}

\frac{d\ket{\psi(\tau)}}{d\tau} = -(\hat{H} - \braket{\hat{H}}) \ket{\psi(\tau)}, 
\end{equation}

\begin{equation}

\ket{\phi(\vec{\theta}(t))} = U(\vec{\theta}(t)) \ket{\phi_0}
\end{equation}

\begin{equation}

U(t) = \exp \left( -i \int_0^t \hat{H}(t) dt \right), 
\end{equation}

\begin{equation}

\hat{H} = \sum_{j=1}^n \hat{H}_j.
\end{equation}

\begin{equation}
\label{eq:STformula}
U(\Delta t) 
= e^{-i \sum_j \hat{H}_j \Delta t}
= \prod_j e^{-i\hat{H}_j\Delta t} + \mathcal{O}((\Delta t)^2).
\end{equation}

\begin{equation}

\lim_{t\to\infty} \frac{\bra{\psi_0} e^{\hat{H}t/2} \hat{H} e^{-\hat{H}t/2} \ket{\psi_0}}{\bra{\psi_0} e^{\hat{H}t} \ket{\psi_0}}
\end{equation}

\begin{gather}

\hat{H} \Psi(\mathbf{r}) = E \Psi(\mathbf{r})
\end{gather}

\begin{gather}

\hat{H} = 
\underbrace{- \sum_i^N \frac{\nabla_i^2}{2}}_{=\hat{H}_K} 
+ \underbrace{\sum_i^N \sum_{j>i}^N \frac{1}{\vert\mathbf{r}_i-\mathbf{r}_j\vert}}_{=\hat{H}_{e-e}}
+ \underbrace{\sum_i^N v(\mathbf{r}_i)}_{=\hat{H}_{e-n}} \\
v(\mathbf{r}_i) = \sum_k^M \frac{z_k}{\vert\mathbf{r}_i-\mathbf{r}_k\vert}
\label{schroedinger_equation}
\end{gather}

\begin{equation}

\Psi(\mathbf{x}_1, ..., \mathbf{x}_i, \mathbf{x}_j, ..., \mathbf{x}_N) = 
-\Psi(\mathbf{x}_1, ..., \mathbf{x}_j, \mathbf{x}_i, ..., \mathbf{x}_N).
\end{equation}

\begin{equation}

\Psi(\mathbf{x}_1, \mathbf{x}_2, ..., \mathbf{x}_N) \neq \psi_1(\mathbf{x}_1) \psi_2(\mathbf{x}_2) ... \psi_N(\mathbf{x}_N)
\end{equation}

\begin{multline}

\Psi(\mathbf{x}_1, \mathbf{x}_2, ..., \mathbf{x}_N) =\\ 
\frac{1}{\sqrt{N!}}
\begin{vmatrix}
\psi_1(\mathbf{x}_1) & \psi_2(\mathbf{x}_1) & ... & \psi_N(\mathbf{x}_1) \\
\psi_1(\mathbf{x}_2) & \psi_2(\mathbf{x}_2) & ... & \psi_N(\mathbf{x}_2) \\
\vdots & \vdots & \ddots & \vdots \\
\psi_1(\mathbf{x}_N) & \psi_2(\mathbf{x}_N) & ... & \psi_N(\mathbf{x}_N)
\end{vmatrix},
\label{slater_determinant}
\end{multline}

\begin{equation}

E_0 = \bra{\Psi_0} \hat{H} \ket{\Psi_0}.
\end{equation}

\begin{equation}

f(x) = \sum_{i=1}^{M}c_{i}\chi_{i}(x).
\end{equation}

\begin{gather}

n(\mathbf{r}) = N \int d^3 r_2 \int d^3 r_3 ... \int d^3 r_N \vert\Psi(\mathbf{r}, \mathbf{r}_2, ..., \mathbf{r}_N)\vert^2
\end{gather}

\begin{align}
\label{HK}
&E_0[n(\mathbf{r})] \nonumber\\
&= \min_{\Psi \to n} \bra{\Psi} \hat{H}_K + \hat{H}_{e-e} + \hat{H}_{e-n} \ket{\Psi} \\
&= \underbrace{\min_{\Psi \to n} \bra{\Psi} \hat{H}_K + \hat{H}_{e-e} \ket{\Psi}}_{=: F[n]} + \int d^3 r n(\mathbf{r}) v(\mathbf{r})
\end{align}

\begin{equation}

-\frac{\nabla^2}{2} \psi_i(\mathbf{r}) + v_{\text{eff}}(\mathbf{r})\psi_i(\mathbf{r}) = \epsilon_i \psi_i(\mathbf{r}).
\end{equation}

\begin{equation}

v_{\text{eff}}(\mathbf{r}) = v_{\text{ext}}(\mathbf{r}) + v_{\text{H}}(\mathbf{r}) + v_{\text{xc}}(\mathbf{r}).
\end{equation}

\begin{equation}
\label{eq:navierstokes}
\frac{\partial\mathbf{u}}{\partial t} = \underbrace{-\mathbf{u}\cdot\nabla\mathbf{u}}_\text{advection} - \nabla p + \underbrace{\frac{1}{\text{Re}}\nabla^2\mathbf{u}}_\text{viscous diffusion}
\end{equation}

\begin{equation}

\nabla\cdot\mathbf{u}
\begin{cases}
= 0, & \text{incompressible flow,} \\
\neq 0, & \text{compressible flow.} 
\end{cases}
\end{equation}

\begin{equation}
\label{eq:lbm}
f_k(\mathbf{x}+\mathbf{e}_k, t+\Delta t) - f_k(\mathbf{x}, t) = 
\Omega(f_k^\text{eq}(\mathbf{x}, t) - f_k(\mathbf{x}, t))
\end{equation}

\begin{equation}
\label{e:lbm}
\frac{\partial F (\mathbf{x},\mathbf{c};t)}{\partial t} + \mathbf{c} \frac{\partial F(\mathbf{x},\mathbf{c};t)}{\partial \mathbf{x}}=0
\end{equation}

\begin{equation}
\label{eq:sph-interpolant}
A_S(\mathbf{r}) = \sum_i m_i \frac{A(\mathbf{r}_i)}{\rho_i} W(\mathbf{r}-\mathbf{r}_i,h)
\end{equation}

\begin{equation}

\sum_i m_i \frac{A(\mathbf{r}_i)}{\rho_i} W(\mathbf{r}-\mathbf{r}_i,h) \to
\langle m A(\mathbf{r})/\rho
\vert W(\mathbf{r},h)
\rangle
\end{equation}

\begin{gather}

\ket{\psi_\text{in}} =
\sum_{k=0}^{\ell-1} \ket{k}^A \ket{0}^B \nonumber\\
\xrightarrow{\text{QRAM}}
\sum_{k=0}^{\ell-1} \ket{k}^A \ket{j_k}^B
= \ket{\psi_\text{out}} \label{eq:qram}
\end{gather}

\begin{gather}

U = \begin{bmatrix} A/\alpha & * \\ * & * \end{bmatrix}
\\
\Updownarrow \nonumber
\\
A = \alpha (\bra{0}^{\otimes a} \otimes I_n) U (\ket{0}^{\otimes a} \otimes I_n), \quad a=m-n.
\end{gather}

