  \begin{theorem}\label{ThmFixIterComp}
Suppose Assumption 3 holds. Choose $\epsilon>0$ and set 
\begin{eqnarray}
\label{stepsizeFixed}
   \alpha&=&\frac{2c\epsilon^{\frac{1}{2\theta}}}{G^2}.
\end{eqnarray}
  \begin{enumerate}
  \item If $0<\theta\leq\frac{1}{2}$, and
   \begin{eqnarray}\label{epsbound}
   0<\epsilon&\leq&\left(\frac{\theta \kappa^2}{2}\right)^{\frac{\theta}{1-\theta}},
   \end{eqnarray}
     then for the iterates of FixedSG,
      $$d(x_{k+1},\calX_h)^2\leq 2\epsilon$$ for all $k\geq K$ where 
   \begin{eqnarray}
  K&\triangleq& 
  \frac{1}{2}\theta \kappa^2 \ln\left(\frac{d(x_1,\calX_h)^2}{\epsilon}\right)\epsilon^{1-\frac{1}{\theta}}
.\nonumber
 \end{eqnarray}
   \item For $\frac{1}{2}\leq \theta\leq 1$, assume $\hat{D}>0$ and $\epsilon>0$ are chosen s.t. 
   \begin{align}\label{DinitBound}
  d(x_1,\calX_h)^2 &\leq \hat{D}
  \\
\epsilon&\leq\min
\left\{\frac{\hat{D}}{2},\left(\frac{\theta \kappa^2}{2}\right)^{2\theta}\hat{D}^{2\theta-1}
\right\}.
\label{Dbound}
    \end{align} 
%   \begin{eqnarray}
%     \text{ and }\epsilon&\leq&
%   \left(\frac{\theta \kappa^2}{2}\right)^{2\theta}\hat{D}^{2\theta-1}.
%   \label{epsBound2a}
%\end{eqnarray}
If $\theta<1$ we further require
\begin{eqnarray} 
         \label{epsBound2}
  \epsilon &\leq&\left(\frac{\kappa^2}{4}\right)^{\frac{\theta}{1-\theta}}
   \end{eqnarray}
  and if $\theta=1$, we require $\kappa\geq 2$. Then
for the iterates of FixedSG, 
$$d(x_{k+1},\calX_h)^2\leq 2\epsilon$$ for all $k\geq K$, where
   \begin{eqnarray}
    \label{requiredK}
       K &\triangleq& 
       \frac{1}{2}\theta\kappa^2 \hat{D}^{1-\frac{1}{2\theta}} \ln\left(\frac{d(x_1,\calX_h)^2}{\epsilon}\right)\epsilon^{-\frac{1}{2\theta}}.
   \end{eqnarray}
  \end{enumerate}
  \end{theorem}
  
  \begin{proof} We consider the two cases, $\theta\leq1/2$ and $\theta\geq 1/2$, separately.
  
  \noindent{\bf\underline{Case 1}: $\boldsymbol{\theta\leq\frac{1}{2}}$.}
  
  \noindent
  From Theorem \ref{ThmFix}, the convergence factor in the constant stepsize case is $q_1=1-\frac{\alpha c}{\theta} e_*^{\frac{1}{2\theta}-1}$ where $e_*=\left(\frac{\alpha G^2}{2c}\right)^{2\theta}=\epsilon$ for this choice of $\alpha$ given in \eqref{stepsizeFixed}. Recall the notation $e_k=d(x_k,\calX_h)^2$. 
  Since $\epsilon$ satisfies (\ref{epsbound}), $0\leq q_1<1$. 
  Thus from Theorem \ref{ThmFix} we know that for all $k\geq 1$
  \begin{align*}
  e_{k+1} - e_*\leq q_1^k(e_1 - e^*)\leq q_1^k e_1
  \end{align*}
  which implies
  \begin{align}\label{eqNewalign}
  \max\{e_{k+1}-e_*,0\}\leq q_1^k e_1.
  \end{align}
  This means that  
  $$
  \ln(\max\{0,e_{k+1}-e_*\})\leq k\ln q_1 + \ln e_1
  $$
  using the convention, $\ln(0)=-\infty$. 
  Thus $e_{k+1}-e_*\leq\epsilon$ is implied by
  $$
  k\ln q_1 + \ln e_1\leq \ln\epsilon
  \iff k\geq \frac{\ln\frac{e_1}{\epsilon}}{\ln\frac{1}{q_1}}.
  $$
%Thus if
 % $$
  %k\geq \frac{\ln\frac{e_1}{\epsilon}}{\ln\frac{1}{|q_1|}}
  %$$
  %then $e_{k+1}-e_*\leq\epsilon$. 
    Now 
  \begin{eqnarray*}
  \ln q_1=\ln\left(1-\frac{\alpha c}{\theta}e_*^{\frac{1}{2\theta}-1}\right)\leq -\frac{\alpha c}{\theta} e_*^{\frac{1}{2\theta}-1}\iff \ln\frac{1}{q_1}\geq \frac{\alpha c}{\theta} e_*^{\frac{1}{2\theta}-1}.
  \end{eqnarray*}
  Therefore if
  \begin{eqnarray*}
  k\geq 
  \frac{\theta\ln\frac{e_1}{\epsilon}}{\alpha c e_*^{\frac{1}{2\theta}-1}}
  =
  \frac{\theta G^2\ln\frac{e_1}{\epsilon}}{2c^2\epsilon^{\frac{1}{\theta}-1}}
  =
  \frac{1}{2}\theta\kappa^2\ln\left(\frac{e_1}{\epsilon}\right)\epsilon^{1-\frac{1}{\theta}}
  \end{eqnarray*}
  then using the fact that for this choice of $\alpha$, $e_*=\epsilon$, we arrive at
  \begin{eqnarray*}
  e_{k+1}\leq e_* +\epsilon = 2\epsilon.
  \end{eqnarray*}
 
  
  
  \noindent{\bf\underline{Case 2}: $\boldsymbol{\theta\geq \frac{1}{2}}$.}
  
  \noindent
  As before, $\alpha = \frac{2c\epsilon^{\frac{1}{2\theta}}}{G^2}$ which implies $e_*=\epsilon$.
  First note that by Part 1 of Theorem \ref{ThmFix}, 
  \begin{eqnarray*}
  d(x_k,\calX_h)^2
  &\leq& 
  \max\{d(x_1,\calX_h)^2,e_*+\alpha^2 G^2\}
  \\
  &=&
  \max\left\{d(x_1,\calX_h)^2,\epsilon+\frac{4 c^2}{G^2}\epsilon^{\frac{1}{\theta}}\right\}
  \\
  &\leq&
  \max\{d(x_1,\calX_h)^2,2\epsilon\}
  \\
  &\leq& \hat{D}
  \end{eqnarray*}
   for all $k\geq 1$, where in the second inequality we used \eqref{DinitBound} and (\ref{epsBound2}) for the case $\theta<1$, and $\kappa\geq 2$ for when $\theta=1$. Therefore $\hat{D}$ is a valid upper bound for the sequence $\{d(x_k,\calX_h)^2\}$ and can be used in place of $D$ in Theorem \ref{ThmFix}. 
    Now from Theorem \ref{ThmFix} the convergence factor is
   \begin{eqnarray*}
   	q_2=1-\frac{\alpha c}{\theta}\hat{D}^{\frac{1}{2\theta}-1}
   \end{eqnarray*}
   which is greater than or equal to $0$ (and less than $1$) because $\epsilon$ satisfies (\ref{Dbound}).
  Recalling (\ref{ghh}) we see that 
  \begin{eqnarray}\label{newcasesss}
  e_{k+1}\leq \max\{e_*+q_2^{k}(d(x_1,\calX_h)^2-e_*),e_*+\alpha^2 G^2\}.
  \end{eqnarray}
  We have already shown that the second argument in the $\max$ above is upper bounded by $2\epsilon$. 
Consider the first argument in the $\max$ in (\ref{newcasesss}). 
 Now $q_2^{k}(d(x_1,\calX_h)^2-e_*)\leq q_2^{k} e_1$, thus
this argument can be dealt with the same way as Case 1 for $\theta\leq1/2$, except for a different convergence factor. 
 Thus we observe
 \begin{eqnarray*}
  \ln q_2=\ln\left(1-\frac{\alpha c}{\theta} \hat{D}^{\frac{1}{2\theta}-1}\right)\leq -\frac{\alpha c}{\theta}  \hat{D}^{\frac{1}{2\theta}-1}\iff \ln\frac{1}{q_2}\geq \frac{\alpha c}{\theta} \hat{D}^{\frac{1}{2\theta}-1}.
  \end{eqnarray*}
  Therefore if 
  \begin{eqnarray*}
  k
  \geq
   \frac{\theta G^2 \hat{D}^{1-\frac{1}{2\theta}}}{2c^2}\ln\left(\frac{e_1}{\epsilon}\right)\epsilon^{-\frac{1}{2\theta}}
  \end{eqnarray*}
 then the first argument in the $\max$ in (\ref{newcasesss}) is upper bounded by $2\epsilon$.

 
% Now consider the second argument in the $\max$ in (\ref{newcasesss}), which is 
% \begin{eqnarray*}
% e_*+\alpha^2 G^2 = \epsilon+\alpha^2 G^2 = \epsilon+\frac{4 c^2}{G^2}\epsilon^{1/\theta}\leq 2\epsilon,
% \end{eqnarray*}
% where we have used again (\ref{epsBound2}) for $\theta<1$ and $\kappa\geq 2$ for $\theta=1$. 
  \end{proof} 