\section{Preliminaries}

\begin{defn} 
Let $(\inspace ,\metric_\inspace ), (\outspace , \metric_\outspace )$ be two metric spaces
$I \subset \inspace$ be an open set. A function $f: \inspace \to \outspace $ is called \emph{H\"older} 
continuous on $I \subset \inspace$ if there exist a \emph{(H\"older) coefficient} $L[I] \geq 0$ and \emph{(H\"older) 
exponent} $p\geq 0$ such that 
\[\forall x,x' \in I : \metric_\outspace \bigl(f(x),f(x')\bigr) \leq L[I] \, \bigl( \metric_\inspace (x,x') \bigr)^p. \]
 \end{defn}
H\"older functions are known to be uniformly continuous. 
A special case of importance is the class of $L$-Lipschitz functions. These are H\"older continuous 
functions with exponent $p=1$. In this context, coeffient $L$ is referred to as Lipschitz constant or number.

\begin{ex}[Square root function]\label{ex:sqrtfctHoelder}
As an example of a H\"older function that is not Lipschitz we can consider $x \mapsto \sqrt(x)$ on domain $I = [0+\epsilon,c]$ where 
$c >\epsilon \geq 0 $. For $\epsilon >0 $ the function is Lipschitz with $L[I] = \sup_{x \in I} \frac{1} {2 \sqrt{x}}$. We can see that the 
coefficient grows inifinitely large as $\epsilon \to 0$. By contrast, the function is H\"older continuous 
with H\"older coefficient $L[I]=1$ and exponent $p=\frac 1 2 $ for any bounded $I \subset \Real$.
We can see this as follows: Let $x,y \in I$ and, without loss of generality,  $y \geq x$. Let $\xi := \sqrt{x}, \gamma := \sqrt{y}$ and thus, $\gamma \geq \xi$. We have:
$\xi \leq \gamma $ $\Leftrightarrow 2 \xi^2 \leq 2\xi\gamma$ $\Leftrightarrow \gamma^2 - 2 \xi\gamma + \xi^2  \leq \gamma^2 - \xi^2$ $\Leftrightarrow (\gamma-\xi)^2  \leq \gamma^2-\xi^2$ $\Leftrightarrow \abs{\gamma-\xi}^2  \leq \abs{\gamma^2-\xi^2}$
 $\Leftrightarrow \abs{\gamma-\xi}  \leq \sqrt{\abs{\gamma^2-\xi^2}}$  $\Leftrightarrow \abs{\sqrt{x}-\sqrt{y}}  \leq \abs{y-x}^{\frac{1}{2}}$. Since, $x,y$ were chosen arbitrarily, we have shown Hoelder continuity as desired.
\end{ex}
 
 In this paper we will consider the special case  $\inspace = \outspace = \Real$ endowed with metric 
 $\metric(x,x') = \abs{x-x'}$.
 Therefore, the H\"older condition becomes 
 \[\forall x,x' \in I : \abs{f(x)-f(x')} \leq L[I] \, \abs{x-x'}^p. \]

\input{content/Ch_kinkyinf/HoelderNLipcontfacts}

\subsection{H\"older continuity of the metric maps}

 
We endeavor to show that $x \mapsto L \norm{ x -s}^p$ is H\"older continuous with coefficient $L$ and exponent $p$. This will become important since these functions will serve as essential building blocks of our conservative H\"older function estimates. 

To this end, we will show that $(x,y) \mapsto \norm{x-y}^p$, for $p \in (0,1] $, is a metric.  This can be utilized to show that
$x \mapsto \norm{ x -s}^p$ is a H\"older continuous function.

To establish the metric property, we note that any positive definite function that is subadditive gives rise to a canonical metric. Formally :


To prove $(x,y) \mapsto \norm{x-y}^p$ is a metric, we need to establish a few facts. 
Firstly, we remind ourselves of the following well-known fact:
\begin{lem} \label{lem:pd_n_concave_subadditive}
 A nonnegative, concave function $g:\Real_{\geq 0} \to \Real$ with $g(0) = 0$ is subadditive. 
 That is, $\forall x,y \in \Real_{\geq 0}: g(x+y) \leq g(x) + g(y)$. 
 
 \begin{proof}
If $x = y = 0$ then subadditivity trivally holds:  $0=g(x+y) \leq g(x) + g(y) = 0$.
So, let $x, y \in \Real_+$ such that $x >0 \vee y >0$.
We have, $g( x +y) = \frac{x}{x+y} g(x+y) + \frac{y}{x+y} g(x+y) \leq g(\frac{x}{x+y} (x+y) ) +  g(\frac{y}{x+y}(x+y)) = g(x) + g(y)$.
Taking into account that $\frac{x}{x+y}, \frac{x}{x+y} \in [0,1]$, the last inequality can be seen as follows:

 Since $g$ is concave we have 
$\forall p \in [0,1], x \in \Real: g(p x) =  g(px + (1-p) 0) \geq p g(x) + (1-p) g(0) \geq p g(x)  $. The last inequality follows from $g(0) \geq 0$.
\end{proof}
\end{lem}

\begin{lem} \label{lem:x2p_pdNsubadd}
 Let $h: \begin{cases} \Real_{\geq 0} \to \Real_{\geq 0},\\ \, x \mapsto x^p\end{cases}$, for $p \in (0,1] $. $h$ is positive definite and subadditive. 
 That is, (i) $h(0) = 0 $ and  $h(x) > 0, \forall x \neq 0$ and (ii) $\forall x,y \in \Real_{\geq 0}: h(x+y) \leq h(x) + h(y)  $.
 Moreover, $h$ is concave. If $p \in (0,1)$, h is strictly concave. 
 
\begin{proof}
\textit{Pos. def. :} $h(0) = 0$.  Also $\lim_{x \to 0_+} h(x) =0$. Since $\nabla h (x) = p h^{p-1}(x) >0 $ for $x >0$, $h$ is strictly monotonically increasing on $\Real_+$. Hence, $h(x) > 0, \forall x >0$. 

\textit{Concavity:} If $p =1$, $h$ is linear and hence, concave. If $p \in (0,1)$, $\nabla^2 h(x) = p (p-1) h(x)^{p-2} > 0$ regardless of $x$.

\textit{Subadditivity:} Follows directly with Lem. \ref{lem:pd_n_concave_subadditive} on the basis of established positive definiteness and concavity.
  
\end{proof}
\end{lem}



\begin{lem}\label{lem:hoeldererror_metric}
Let $p \in (0,1]$.
With definitions as in Thm. \ref{thm:subaddmetric1}, we assume that set $G$ is endowed with a quasi- metric $d$. Function
$\metric: \begin{cases} \inspace \times \inspace \to \Real_{\geq 0} \\ (x,y) \mapsto \Bigl(d(x,y)\Bigr)^p \end{cases}$ is a quasi-metric on $G$.
If $d$ is a metric then so is $\metric$.
\begin{proof}
 By Lem. \ref{lem:x2p_pdNsubadd}, $x\mapsto x^p$ is pos. def. and subadditive. Therefore, positive definiteness and the triangle inequality of $d$ readily extend to $\metric$ as follows: 

\textit{Pos. def.:}
Let $x=0$. $\metric(x,x) = d(x,x)^p = 0^p = 0$. If $x \neq 0$ then $k :=d(x,x) \neq 0$. Hence   $\metric(x,x) = d(x,x)^p = k^p \neq 0$.

\textit{Triangle inequality:}
Choose arbitrary $x,y,z \in \inspace $. We have $\metric(x,z) = d(x,z)^p \leq (d(x,y) + d(y,z) \bigr)^p \leq d(x,y)^p + d(y,z)^p = \metric(x,y) + \metric(y,z)$. Here, the first inequality followed from the triangle inequality of quasi-metric $d$ and the second from subadditivity properties established in Lem. \ref{lem:x2p_pdNsubadd}.

\textit{Symmetry:} If $d$ is a metric it is symmetric. Hence, $\metric(x,y) = d(x,y)^p = d(y,x)^p = \metric(y,x), \forall x,y \in \inspace $ in which case $\metric$ also is symmetric.
\end{proof}
\end{lem}

Before proceeding we establish a slight generalization of the well-known \textit{reverse triangle inequality}:

\begin{lem}[Reverse Triangle Inequality] \label{thm:revtriangle}
Let  $\inspace$ be a set and $\metric : \inspace^2 \to \Real$ a symmetric function that fulfills the triangle inequality. 
That is,  $\forall x,y,z \in \inspace: \metric (x,y) = \metric(y,x) \wedge \metric(x,z) \leq \metric(x,y) + \metric(y,z)$.

Then \[\forall x,y,z \in \inspace: \abs{\metric(x,y) - \metric(z,y)} \leq \metric(x,z).\]
\begin{proof}

For contradiction, assume 
$\abs{\metric(x,y) - \metric(z,y)}>\metric(x,z)$ for some $x,y,z \in \inspace$.
This is implies  
$
(i)\,\,\, \metric(x,y) - \metric(z,y)>\metric(x,z) 
\, \, $  or  $
  \,\,  (ii) \,\,\,\, \metric(z,y)-\metric(x,y) >\metric(x,z)$.
Both inequalities contradict the triangle inequality:
$(i) \Leftrightarrow \metric(x,y)  >\metric(x,z) \metric(z,y) $ and 
$(ii) \Leftrightarrow  \metric(z,y) > \metric(x,z) + \metric(x,y) =  \metric(z,x) + \metric(x,y)$.

\end{proof}
\end{lem}


\begin{thm}
Let $\metric$ be a metric on set $G$. For arbitrary $s \in \inspace $ we define $\phi_s: \inspace \to \Real $ as $\phi_s: x \mapsto \metric (x,s) $.
$\phi_s $ is Lipschitz with respect to metric $\metric$. That is, \[\forall x,y \in \inspace : \abs{\phi_s(x) - \phi_s(y) } \leq \metric (x,y). \]
\begin{proof}
$\abs{\phi_s(x) - \phi_s(y)} = \abs{\metric(x,s) - \metric(y,s)} \stackrel{Thm. \ref{thm:revtriangle}} {\leq} \metric(x,y), \forall x,y,s \in \inspace $.
\end{proof}
\end{thm}
Finally, combining this theorem with Lem. \ref{lem:hoeldererror_metric} immediately establishes that mappings of the form $\metric(\cdot,s)^p$ and hence, of the form
$\norm{\cdot -s}^p$ are H\"older continuous with exponent $p$ ($\in (0,1]$):

\begin{thm}\label{thm:pmetricphoelder}
Let $\metric$ be a metric on set $G$ and let $p \in (0,1], L \geq 0$. For arbitrary $s \in \inspace $ we define $\phi_s:\begin{cases}  \inspace \to \Real \\ x \mapsto L \, \bigl(\metric (x,s) \bigr)^p\end{cases}$, where 
$\phi_s $ is H\"older with exponent $p$. That is, \[\forall x,y \in \inspace : \abs{\phi_s(x) - \phi_s(y) } \leq L \, \metric (x,y)^p. \]
In particular, for any norm $\norm \cdot$ on $G$ and $s \in \inspace $, mapping $x \mapsto L \norm{x-s}^p$ is H\"older with constant $L$ and exponent $p$.
\begin{proof}
By Lem. \ref{lem:hoeldererror_metric}, $\metric(\cdot,\cdot)$ is a metric on $G$. Hence, Lem. \ref{thm:revtriangle} is applicable yielding:
$\abs{\phi_s(x) - \phi_s(y)} = L \, \abs{\metric(x,s)^p - \metric(y,s)^p} \stackrel{Lem. \ref{thm:revtriangle} } {\leq} \metric(x,y)^p, \forall x,y,s \in \inspace$. The last sentence concerning the norms follows from the fact that a mapping $(x,y) \mapsto \norm{x-y}$ defines a metric.
\end{proof}
\end{thm}



 At first glance, the result may seem intuitive. However, it should be noted that, for $p >1$, $x \mapsto \norm{x -s}^p$ is no longer H\"older with exponent $p$. This is consistent with the well-known fact that H\"older functions with exponent $>1$ are constant functions. 
%We conclude this section by the following theorem stating that any concatenation of Hoelder continuous functions is Hoelder continuous:
%
%\begin{thm} \label{thm:concathoelder}
%Let $(\statespace, \metric)$ be a metric space and $f,g : \statespace \to \statespace$ be two Hoelder continuous mappings with Hoelder constants $L_f, L_g$ and Hoelder exponents $p_f,p_g$, respectively.
%Then, the concatenation $h=f \circ g: \statespace \to \statespace $ is also Hoelder continuous with Hoelder constant $L_h:= L_f L_g^{p_f}$ and exponent $p_h:=p_g \, p_f$.
%That is, 
%\[\forall \state,\state' \in \statespace: \metric\bigl(h(\state),h(\state')\bigr) \leq L_h \bigl(\metric(\state,\state')\bigr)^{p_h}.\]
%\begin{proof}
%%\begin{align}
%$\metric\bigl(f \circ g(\state),f\circ g(\state')\bigr) \leq L_f  \Bigl(\metric(g(\state),g(\state'))\Bigr)^{p_f}$
%$\leq L_f  \Bigl(L_g \metric(\state,\state')^{p_g}\Bigr)^{p_f}$ $= L_f L_g^{p_f}   \Bigl(\metric(\state,\state')\Bigr)^{p_g\, p_f} $ where in the first step we were using Hoelder-continuity of $f$ and in the second, we were using Hoelder continuity of $g$ combined with the fact that $(\cdot)^{p_f}$ is a monotonically increasing  function. 
%
%\end{proof}
%\end{thm} 
%In conjunction with Hoelder properties of the square root function established in Ex. \ref{ex:sqrtfctHoelder}, Thm. 
%\ref{thm:concathoelder} immediately yields the following result:
%\begin{cor}
%If $f: \statespace \to \statespace $ is Hoelder continuous with constant $L_f$ and exponent $p_f$ then $\sqrt{f}$ also is Hoelder, having  Hoelder constant $\sqrt{L_f}$ and exponent $p_f$.
%\end{cor}

