\subsection{Resolvent equations}

Separation of variables based on the eigensystem of $\mathcal{A}$ yields a solution representation
\[
u(x,t)=\sum_{n=1}^\infty \Bigl(
\sigma(t)w_{fn}(t)\langle f,\varphi_n\rangle 
+w_{2n}(t)\langle u_2,\varphi_n\rangle 
+w_{1n}(t)\langle u_1,\varphi_n\rangle 
+w_{0n}(t)\langle u_0,\varphi_n\rangle
\Bigr)\varphi_n(x)
\]
and convergence of the sums is guaranteed by the energy estimates from Theorem~\ref{thm:sumfrac}.
Here $w_{fn}$, $w_{2n}$, $w_{1n}$, $w_{0n}$ denote the solutions of the
resolvent equation
\[
\begin{aligned}
&w_{n,tt}+c^2\lambda_n w_n
+\sum_{j=1}^J d_j D_t^{2+\gamma_j}w_n
+\sum_{k=1}^N b_k\lambda_n^{\beta_k} D_t^{\alpha_k} w_n = 
\begin{cases}1\ \mbox{ for }w_{fn}\\0\ \mbox{ else}\end{cases}\\
&
w_{n,tt}(0)=\begin{cases}1\ \mbox{ for }w_{2n}\\0\ \mbox{ else}\end{cases}, \quad
w_{n,t}(0)=\begin{cases}1\ \mbox{ for }w_{1n}\\0\ \mbox{ else}\end{cases}, \quad
w_{n}(0)=\begin{cases}1\ \mbox{ for }w_{0n}\\0\ \mbox{ else}\end{cases}.
\end{aligned}
\]

From the Laplace transformed resolvent equations we obtain the resolvent solutions
\[ \begin{aligned}
&\hat{w}_{fn}(s)=\frac{1}{
\omega(s;\lambda_n)}
\,, \quad
\hat{w}_{0n}(s)=
\frac{s+\sum_{j=1}^J d_j s^{\gamma_j+1}+\sum_{k=1}^N s^{\alpha_k-1} b_{k}\lambda_n^{\beta_{k}}}{
\omega(s;\lambda_n)}
=\frac{\omega(s,\lambda_n)-c^2\lambda_n}{s\omega(s;\lambda_n)}
\,, \\
&\hat{w}_{1n}(s)=\frac{1+\sum_{j=1}^J d_j s^{\gamma_j}}{
\omega(s;\lambda_n)}
\,, \quad
\hat{w}_{2n}(s)=\frac{\sum_{j=1}^J d_j s^{\gamma_j-1}}{
\omega(s;\lambda_n)}
\end{aligned}\]
with 
\[
\omega(s;\lambda_n)=s^2+c^2\lambda_n+\sum_{j=1}^J d_j s^{\gamma_j+2}+\sum_{k=1}^N s^{\alpha_k} b_{k}\lambda_n^{\beta_{k}},
\]
where $\hat{w}$ denotes the Laplace transform of $w$.

Formally we can write
\[
\hat{u}(x,s)=\sum_{n=1}^\infty \Bigl(
\hat{\sigma}(s)\hat{w}_{fn}(s)\langle f,\varphi_n\rangle 
+\hat{w}_{2n}(s)\langle u_2,\varphi_n\rangle 
+\hat{w}_{1n}(s)\langle u_1,\varphi_n\rangle 
+\hat{w}_{0n}(s)\langle u_0,\varphi_n\rangle
\Bigr)\varphi_n(x)
\]
and therefore
\[
\widehat{B_iu}(s)=\sum_{n=1}^\infty \Bigl(
\hat{\sigma}(s)\hat{w}_{fn}(s)\langle f,\varphi_n\rangle 
+\hat{w}_{2n}(s)\langle u_2,\varphi_n\rangle 
+\hat{w}_{1n}(s)\langle u_1,\varphi_n\rangle 
+\hat{w}_{0n}(s)\langle u_0,\varphi_n\rangle
\Bigr)B_i\varphi_n\,.
\]

