\section{Completion of the Proof of Lemma \ref{lem4}}\label{sec:app_d}

Let $p_1 \in (0,1)$, and let $N^{(n)}$ be a random variable as above, i.e., $N^{(n)}  \rightarrow \infty$ as $n \rightarrow \infty$. Consider the sequence of independent random variables $Y_u \sim Bernoulli (p_u)$ for $u=1, 2, \cdots, N^{(n)}$ such that
\begin{enumerate}
	\item For all $n$ and all $u \in \left\{1, 2, \cdots, N^{(n)}\right\}$, $\abs*{p_u-p_1} \leq \zeta_n.$
	\item $\lim\limits_{n\to\infty} \zeta_n =0.$
\end{enumerate}
Define
\[\overline{Y}\triangleq \frac{1}{N^{(n)}}\sum_{u=1}^{N^{(n)}}Y_u,\]
then $\overline{Y} \xrightarrow{d} p_1.$

\begin{proof}
Note
\begin{align}
\no E[\overline{Y}] &= \frac{1}{N^{(n)}}\sum_{u=1}^{N^{(n)}}p_u\\
\nonumber &\leq \frac{1}{N^{(n)}} \sum_{u=1}^{N^{(n)}}\left(p_1+\zeta_n\right)\\
\nonumber &= \frac{1}{N^{(n)}}\cdot N^{(n)}(p_1+\zeta_n) \\
\nonumber &= p_1+\zeta_n. \ \
\end{align}

Similarly we can prove $E\left[\overline{Y}\right]\geq p_1-\zeta_n$. Since as $n$ becomes large, $\zeta_n\rightarrow 0$ and $p_1 \in (0,1)$, we can conclude
\begin{align}\label{eq:H4}
\lim\limits_{n\to\infty} E\left[\overline{Y}\right]=p_1.
\end{align}
Also,
\begin{align}
	\no Var\left(\overline{Y}\right) &= \frac{1}{\left(N^{(n)}\right)^2}\sum_{u=1}^{N^{(n)}}p_u\left(1-p_u\right) \\
	\nonumber &\leq \frac{1}{(N^{(n)})^2} \sum_{u=1}^{N^{(n)}}\left(p_1+\zeta_n\right)\left(1-p_1+\zeta_n\right)\\
	\nonumber &= \frac{1}{(N^{(n)})^2}\cdot N^{(n)}\left(p_1+\zeta_n\right)\left(1-p_1+\zeta_n\right) \\
	\nonumber &= \frac{1}{N^{(n)}} \left(p_1+\zeta_n\right)\left(1-p_1+\zeta_n\right). \ \
\end{align}
Thus,
\begin{align}\label{eq:H5}
\lim_{n\to\infty} Var\left(\overline{Y}\right)=0.
\end{align}
By using (\ref{eq:H4}), (\ref{eq:H5}), and Chebyshev's inequality, we can conclude
\[\overline{Y}\xrightarrow{d} p_1.\]

\end{proof}
