\noindent\textbf{Proof of \ref{prop::amm1}.\;}  We will prove $F^{\ak}\leq \lF^{\ak}$ and $\lF^{\akp}\leq \lF^{\ak}$ by induction, from which it can be shown that $\sF^{(\skp)}\leq \sF^{(\sk)}$.
\begin{enumerate}[leftmargin=0.5cm]
	\item From lines~\ref{line::alg5::Fakp2}, \ref{line::alg5::lFa0}, \ref{line::alg5::Fakp1}, \ref{line::alg5::lFakp} of \cref{algorithm::amm}, it can be shown that 
	\begin{equation}
		\nonumber
		F^{\alpha(-1)}=F^{\alpha(0)}=\lF^{\alpha(-1)}=\lF^{\alpha(0)}.
	\end{equation}
	\item Suppose $\sk\geq 0$ and $F^{\ak}\leq \lF^{\ak}$ holds at $\sk$-th iteration. In terms of $\Xakh$, if the adaptive restart scheme  for $\Xakh$ is not triggered, it is immediate to show from line~\ref{line::alg6::restart1} of \cref{algorithm::amm_x} that
	\begin{equation}\label{eq::GGHFk2}
		\sG^{\akh}  \leq \lF^{\ak}.
	\end{equation}
	On the other hand, if the adaptive restart scheme for $\Xakh$ is triggered, line~\ref{line::alg6::Xakh2} of \cref{algorithm::amm_x} results in
	\begin{multline}\label{eq::GHHk}
	 G^{\alpha}(\Xakh|\Xk) \leq	H^{\alpha}(\Xakh|\Xk)\leq\\  H^{\alpha}(\Xak|\Xk) = 0,
	\end{multline}
	where the first inequality and the last equality are due to \cref{lemma::lG}\ref{lemma::lGd} and \cref{eq::lGMa}, respectively. From \cref{eq::Gakp,eq::GHHk}, we obtain
	\begin{multline}\label{eq::GGHFk}
	\!\!\!G^{\akh} = G^\alpha(\Xakh|\Xk) + F^{\ak}\leq\\
	 H^\alpha(\Xakh|\Xk) + F^{\ak}\leq F^{\ak}\leq \sF^{\ak}.
	\end{multline}
	Therefore, no matter whether the adaptive restart scheme is triggered or not, we conclude from \cref{eq::GGHFk,eq::GGHFk2} that
	\begin{equation}\label{eq::GHlF}
		G^{\akh}\leq  \lF^{\ak}
	\end{equation}
	always holds. Furthermore, if $\Xakp$ and $G^{\akp}$ result from line~\ref{line::alg6::Xakp3} of \cref{algorithm::amm_x}, we obtain $\Xakp=\Xakh$ and $G^{\akp}=G^{\akh}$, which and \cref{eq::GHlF} yield
	\begin{equation}\label{eq::GlFbnd2}
		G^{\akp}=G^{\akh}\leq \lF^{\ak}.
	\end{equation}
	Otherwise, line~\ref{line::alg6::check1} of \cref{algorithm::amm_x} and \cref{eq::GHlF} suggest
	\begin{equation}\label{eq::GlFbnd}
		G^{\akp} - \lF^{\ak} \leq \phi\cdot \big(\sG^{\akh}-\lF^{\ak}\big)\leq 0.
	\end{equation}
	Then, \cref{eq::GlFbnd,eq::GlFbnd2} suggest
	\begin{equation}\label{eq::GkpFk}
		G^{\akp} \leq \lF^{\ak}
	\end{equation}
	always holds, from which and \cref{prop::FsF}\ref{prop::FsF4} we conclude
	\begin{equation}\label{eq::FlFak}
		F^{\akp}\leq \lF^{\akp}\leq \lF^{\ak}.
	\end{equation}
	\item Therefore, it can be concluded that $F^{\ak}\leq \lF^{\ak}$ and  $\lF^{\akp}\leq \lF^{\ak}$.
\end{enumerate}
Summing both sides of  $\sF^{\akp}\leq \sF^{\ak}$ over all the nodes $\alpha$ and implementing Propositions \ref{prop::FsF}\ref{prop::FsF1} and \ref{prop::FsF}\ref{prop::FsF2} yields
\begin{equation}
	\nonumber
	\lF^{(\skp)}=\sum_{\alpha\in\AA}\lF^{\akp} \leq \sum_{\alpha\in\AA}\lF^{\ak}=\lF^{(\sk)},
\end{equation}
which suggests that $\lF^{(\sk)}$ is nonincreasing. The proof is completed.


\vspace{0.8em}
\noindent\textbf{Proof of \ref{prop::amm2}.\;} Recalling that $F(\Xk)\geq 0$ holds  by definition for any $\sk\geq 0$ and $\lF^{(\sk)}$ is the exponential moving average of $F(X^{(0)}),\,F(X^{(1)}),\,\cdots,\, F(\Xk)$, we obtain $\sF^{(\sk)}\geq 0$, i.e., $\sF^{(\sk)}$ is bounded below. In addition, \cref{prop::amm}\ref{prop::amm1} indicates that $\lF^{(\sk)}$ is nonincreasing, and thus, there exists $F^{\infty}$ such that $\lF^{(\sk)}\rightarrow F^{\infty}$, from which and \cref{eq::lFk} it can be concluded that $F(\Xk)\rightarrow F^{\infty}$ as well. The proof is completed.


\vspace{0.8em} 
\noindent\textbf{Proof of \ref{prop::amm3}.\;} From \cref{eq::G2}, it can be shown that $G(\Xkp|\Xk)$ takes the form as
\begin{equation}
	\nonumber
	\begin{aligned}
	G(\Xkp|\Xk) =& \sum_{\alpha\in\AA}G^\alpha(\Xak|\Xk) + F(\Xk)\\
	=&\sum_{\alpha\in\AA}G^\alpha(\Xak|\Xk) +\!\sum_{\alpha\in\AA} F^{\ak},
	\end{aligned}
\end{equation}
where the last equality is due to \cref{prop::FsF}\ref{prop::FsF1}. Applying \cref{eq::Gakp} on the equation above results in
\begin{equation}\label{eq::Gk}
G(\Xkp|\Xk)=\sum_{\alpha\in\AA} G^{\akp}.
\end{equation}
Recalling $G^{\akp}\leq \lF^{\ak}$ from \cref{eq::GkpFk} and $\sum_{\alpha\in\AA}\lF^{\ak} = \lF^{(\sk)}$ from \cref{prop::FsF}\ref{prop::FsF2}, we obtain
\begin{equation}\label{eq::GlFk}
	G(\Xkp|\Xk) = \sum_{\alpha\in\AA} G^{\akp} \leq \sum_{\alpha\in\AA} \lF^{\ak} = \lF^{(\sk)}.
\end{equation}
From \cref{eq::GlFk}, it can be shown that
\begin{equation}\label{eq::lFFG}
	\lF^{(\sk)} - F(\Xkp)\geq G(\Xkp|\Xk) - F(\Xkp).
\end{equation}
Substitute \cref{eq::Gxkp,eq::Fxkp} into the right-hand side of \cref{eq::lFFG} and simplify the resulting equation:
\begin{multline}\label{eq::lFkFkp2}
	\lF^{(\sk)} - F(\Xkp)\geq \frac{1}{2}\|\Xkp-\Xk\|_{\nGammak}^2-\\
	\frac{1}{2}\|\Xkp-\Xk\|_{\nMk}^2.
\end{multline}
From \cref{eq::lFkFkp2,eq::lFklFkp}, we obtain
\begin{multline}
	\nonumber
	\lF^{(\sk)}-\lF^{(\skp)}= \eta\cdot\big(\lF^{(\sk)}-F^{(\skp)}\big)\geq\\
	\frac{\eta}{2}\|\Xkp-\Xk\|_{\nGammak}^2-\frac{\eta}{2}\|\Xkp-\Xk\|_{\nMk}^2.
\end{multline}
From \cref{eq::GMk}, note that $\nGammak-\nMk\geq \xi\cdot\I$, and thus, there exists $\delta > 0$ such that the equation above is reduced to
\begin{equation}\label{eq::lFkFkp}
	\lF^{(\sk)} - \lF^{(\skp)} \geq \frac{\delta}{2}\|\Xkp-\Xk\|^2
\end{equation}
as long as $\xi>0$. Furthermore, \cref{prop::amm}\ref{prop::amm2} yields $$\lF^{(\sk)}-\lF^{(\skp)}\rightarrow 0,$$ from which and \cref{eq::lFkFkp}, we obtain
\begin{equation}\label{eq::XkpXk}
	\|\Xkp-\Xk\|\rightarrow 0.
\end{equation}
The proof is completed.

\vspace{0.8em} 
\noindent\textbf{Proof of \ref{prop::amm4}.\;} In terms of $\Xakh$, there are two possible cases:
\begin{enumerate}[leftmargin=0.45cm]
\item If $\Xakh$ is from line~\ref{line::alg6::Xakh1} of \cref{algorithm::amm_x}, then line~\ref{line::alg6::restart1} of \cref{algorithm::amm_x} indicates
\begin{equation}\label{eq::lFG1}
\sF^{\ak}-G^{\akh}\geq  \psi\cdot\|\Xakh-\Xak\|^2.
\end{equation}
\item If $\Xakh$ is from line~\ref{line::alg6::Xakh2} of \cref{algorithm::amm_x}, then note that \cref{eq::GGHFk} holds for any $\sk\geq 0$, which suggests
\begin{multline}
\nonumber
\sF^{\ak}-G^{\akh}\geq H^\alpha(\Xakh|\Xk)-\\
G^\alpha(\Xakh|\Xk).
\end{multline}
Recalling the definitions of $G^\alpha(\Xakh|\Xk)$ and $H^\alpha(\Xakh|\Xk)$ in \cref{eq::GMa,eq::lGMa}, we rewrite the equation above as
\begin{multline}\label{eq::lFG}
\sF^{\ak}-G^{\akh}\geq \frac{1}{2}\|\Xakh-\Xak\|_{\lnGammaak}^2-\\
\frac{1}{2}\|\Xakh-\Xak\|_{\nGammaak}^2.
\end{multline}
Similar to $\nGammak$ and $\lnGammak$ in \cref{eq::lGGk}, we obtain
\begin{equation}\label{eq::lGGak}
\lnGammaak \succeq \nGammaak + (\zeta-\xi)\cdot\I.
\end{equation}
Applying \cref{eq::lGGak} on the right-hand side of \cref{eq::lFG} indicates
\begin{multline}\label{eq::lFG2}
	\sF^{\ak}-G^{\akh}\geq \frac{\zeta-\xi}{2}\|\Xakh-\Xak\|^2.
\end{multline}
\end{enumerate}
Then, as a result of \cref{eq::lFG1,eq::lFG2}, there exists a constant scalar $\sigma'>0$ such that
\begin{equation}\label{eq::lFG3}
	\sF^{\ak}-G^{\akh}\geq \frac{\sigma'}{2}\|\Xakh-\Xak\|^2
\end{equation}
if $\zeta>\xi>0$. In addition, lines~\ref{line::alg6::check1} to \ref{line::alg6::check2} of \cref{algorithm::amm_x} results in
\begin{multline}\label{eq::lFGak2}
\sF^{\ak} - \sG^{\akp} \geq \phi\cdot \Big(\sF^{\ak} - \sG^{\akh}\Big)\geq\\
\frac{\phi\sigma'}{2}\|\Xakh-\Xak\|^2,
\end{multline}
where the last inequality is from \cref{eq::lFG3}. Summing both sides of \cref{eq::lFGak2} over all the nodes $\alpha\in\AA$ and simplifying the resulting equation with \cref{prop::FsF}\ref{prop::FsF2} and \cref{eq::Gk}, we obtain
\begin{equation}
\nonumber
\sF^{(\sk)} - G(\Xkp|\Xk) \geq \frac{\phi\sigma'}{2}\|\Xkh-\Xk\|^2.
\end{equation}
Recalling $G(\Xkp|\Xk)\geq F(\Xkp)$  from \cref{prop::G}\ref{prop::G2}, the equation above indicates
\begin{multline}\label{eq::lFF}
\sF^{(\sk)} - F(\Xkp) \geq \sF^{(\sk)} - G(\Xkp|\Xk) \geq\\ \frac{\phi\sigma'}{2}\|\Xkh-\Xk\|^2.
\end{multline}
From \cref{eq::lFF,eq::lFklFkp}, it is immediate to show
\begin{multline}
\nonumber
\sF^{(\sk)} - \sF^{(\skp)} \geq \eta\cdot\Big(\sF^{(\sk)}-F(\Xkp)\Big)\geq \\
\frac{\eta\phi\sigma'}{2}\|\Xkh-\Xk\|^2.
\end{multline}
Therefore, there exists a constant scalar $\delta'>0$ such that
\begin{equation}
\sF^{(\sk)} - \sF^{(\skp)} \geq \frac{\delta'}{2}\|\Xkh-\Xk\|^2.
\end{equation}
Since $\sF^{(\sk)} \rightarrow F^{\infty}$, it can be concluded that
\begin{equation}
	\|\Xkh-\Xk\|\rightarrow 0
\end{equation}
if $\zeta>\xi>0$. The proof is completed.
\vspace{0.8em} 

\noindent\textbf{Proof of \ref{prop::amm5} and \ref{prop::amm6}.\;} The proofs of Propositions \ref{prop::amm}\ref{prop::amm5} and \ref{prop::amm}\ref{prop::amm6} are almost the same as these of Propositions \ref{prop::ammc}\ref{prop::ammc5} and \ref{prop::ammc}\ref{prop::ammc6}, which are thus omitted due to space limitation.
