\section{Direct scattering transform}\label{s scatt}
For a review of the scattering map for the DNLS equation we are going to follow closely \cite{Pelinovsky2016,Liu2016}. As pointed out in the pioneer work \cite{KaupNewell1978}, the DNLS equation is the compatibility condition for solutions $\psi\in\Compl^2$ of the linear system given by
\begin{equation}\label{e Lax1}
    \partial_x\psi=[-\ii\lambda^2\sigma_3+\lambda Q(u)]\psi
\end{equation}
and
\begin{equation}\label{e Lax2}
    \partial_t\psi=[-2\ii\lambda^4\sigma_3+ 2\lambda^3 Q(u)+\ii\lambda^2|u|^2\sigma_3- \lambda |u|^2Q(u) +\ii\lambda \sigma_3 Q(u_x)]\psi,
\end{equation}
where
\begin{equation*}
    Q(u)=
    \left[
      \begin{array}{cc}
        0 & u(x,t) \\
        -\overline{u}(x,t) & 0 \\
      \end{array}
    \right],\qquad
    \sigma_3=
    \left[
      \begin{array}{cc}
        1 & 0 \\
        0 & -1 \\
      \end{array}
    \right].
\end{equation*}
In this context the term \emph{compatibility condition} is chosen, because if the spectral parameter $\lambda$ is independent of $x$ and $t$, it can be shown that the formal equality of the mixed derivatives, $\partial_x\partial_t\psi=\partial_t\partial_x\psi$,  is equivalent to the statement that $u$ solves the DNLS equation (\ref{e dnls}).
\input{jost_functions}
\input{scattering_data}
%\input{g}




%$\lambda_k\in\Compl_{I}\footnote{$\Compl_{I}:=\set{\eta+\ii \zeta\in\Compl:\eta,\zeta>0}$}$ $(k=1,...,N)$, $z_k:=\lambda_k^2\in\Compl_+$, $c_k\in\Compl^*$, $r_{\pm}\in L^{2,1}(\Real)$
%\begin{samepage}
%\begin{framed}
%\textbf{RHP[DNLS]:}\\Find for each $(x,t)\in\Real\times\Real$ a $2\times 2$-matrix valued function $\Compl\ni z\mapsto m(z;x,t)$ which satisfies
%\begin{enumerate}[(i)]
%  \item $m(z;x,t)$ is meromorphic in $\Compl\setminus\Real$ (with respect to the parameter $z$).
%  \item $m(z;x,t)=1+\mathcal{O}\left(\frac{1}{z}\right)$ as $|z|\to\infty$.
%  \item The non-tangential boundary values $m_{\pm}(z;x,t)$ exist for $z\in\Real$ and satisfy the jump relation
%      \begin{equation}\label{e jump}
%        m_+=m_-(1+R),\quad\text{where }
%        R(z;x,t):=
%        \left(
%          \begin{array}{cc}
%            \overline{r}_+(z)r_-(z) & e^{\overline{\phi}(z)}\overline{r}_+(z) \\
%            e^{\phi(z)}r_-(z) & 0 \\
%          \end{array}
%        \right)
%      \end{equation}
%      with
%      \begin{equation}\label{e def phase}
%         \phi(z):=2\ii xz+4\ii z^2t.
%      \end{equation}
%  \item $m$ has simple poles at $z_1,...,z_N,\overline{z}_1,...,\overline{z}_N$ with
%      \begin{equation}\label{e Res}
%        \left[\begin{aligned}
%          \res_{z=z_k}m(z;x,t)&=\lim_{z\to z_k}m(z;x,t)
%          \left(
%            \begin{array}{cc}
%              0 & 0 \\
%              2\ii\lambda_kc_k e^{\phi_k} & 0
%            \end{array}
%          \right),\\
%          \res_{z=\overline{z_k}}m(z;x,t)&=\lim_{z\to \overline{z}_k}m(z;x,t)
%          \left(
%            \begin{array}{cc}
%              0 & \frac{-\overline{c}_k}{2\ii\lambda_k} e^{\overline{\phi}_k} \\
%              0 & 0
%            \end{array}
%          \right).
%        \end{aligned}\right.
%      \end{equation}
%\end{enumerate}
%\end{framed}
%\end{samepage}
%\begin{rem}\label{r uniqueness + det=1}
%    Without further theory we can observe that if \textbf{RHP[DNLS]} is solvable, then the solution is unique. In order to show the uniqueness of solutions, we firstly find the following (trivial) Riemann Hilbert problem for the map $z\mapsto \det(m(z;x))$:
%    \begin{equation*}
%        \left\{
%           \begin{array}{ll}
%             \det(m(z;x))\text{ is an entire function with respect to the parameter }z,\\
%             \det(m(z;x))\to 1,\text{ as }|z|\to\infty.
%           \end{array}
%         \right.
%    \end{equation*}
%    By Liouville's theorem we conclude
%    \begin{equation}\label{e det m=1}
%        \det(z;x)\equiv 1,\text{ for all }x\in\Real\text{ and }z\in \Compl.
%    \end{equation}
%    Hence, for a possible solution $m$ of \textbf{RHP[DNLS]}, $[m(z;x)]^{-1}$ exists for all $x\in\Real$ and $z\in \Compl$. If we have second solution $\widetilde{m}(z;x)$, the ratio $\widetilde{m}(z;x)[m(z;x)]^{-1}$ satisfies
%    \begin{equation*}
%        \left\{
%           \begin{array}{ll}
%             \widetilde{m}(z;x)[m(z;x)]^{-1}\text{ is an entire function with respect to the parameter }z,\\
%             \widetilde{m}(z;x)[m(z;x)]^{-1}\to 1,\text{ as }|z|\to\infty,
%           \end{array}
%         \right.
%    \end{equation*}
%    such that $\widetilde{m}(z;x)[m(z;x)]^{-1}\equiv 1$.
%\end{rem}



