\section{Proofs from \Cref{sec:estimation}}
For convenience, throughout this section we will use the notation:
\begin{align}
    \Psi(a, f) :=~& \E\brk*{m(Z; f) - a(X)\cdot f(X)} = \E[(a_0(X)-a(X))\, f(X)] \tag{by Riesz definition}\\
    \Psi_n(a, f) :=~& \frac{1}{n}\sum_{i=1}^{n} \left(m(Z_i; f) - a(X_i)\cdot f(X_i)\right)
\end{align}

\subsection{Proof of \Cref{thm:reg-main-error}}

\begin{proof} 
Let:
\begin{align}
    \Psi_n^\lambda(a, f) =~& \Psi_n(a, f) - \|f\|_{2,n}^2 - \lambda \|f\|_{\mcA}^2\\
    \Psi^{\lambda}(a, f) =~& \Psi(a, f) - \frac{1}{4} \|f\|_2^2 - \frac{\lambda}{2}\|f\|_{\mcA}^2
\end{align}
Thus our estimate can be written as:
\begin{equation}
    \hat{a} := \argmin_{a\in \mcA} \sup_{f\in \mcF} \Psi_n^{\lambda}(a, f) + \mu \|a\|_{\mcA}^2
\end{equation}


\paragraph{Relating empirical and population regularization.} 
As a preliminary observation, we have that by Theorem 14.1 of \cite{wainwright2019high}, w.p. $1-\zeta$:
\begin{equation}
    \forall f\in \mcF_{B}: \left|\|f\|_{n,2}^2 - \|f\|_2^2 \right| \leq \frac{1}{2} \|f\|_2^2 + \delta^2 
\end{equation}
for our choice of $\delta:=\delta_n + c_0 \sqrt{\frac{\log(c_1/\zeta)}{n}}$, where $\delta_n$ upper bounds the critical radius of $\mcF_{B}$ and $c_0, c_1$ are universal constants. Moreover, for any $f$, with $\|f\|_{\mcA}^2\geq B$, we can consider the function $f \sqrt{B}/\|f\|_{\mcA}$, which also belongs to $\mcF_{B}$, since $\mcF$ is star-convex. Thus we can apply the above lemma to this re-scaled function and multiply both sides by $\|f\|_{\mcA}^2/B$, leading to:
\begin{equation}
    \forall f\in \mcF \text{ s.t. } \|f\|_{\mcA}^2 \geq B: \left|\|f\|_{n,2}^2 - \|f\|_2^2 \right| \leq \frac{1}{2} \|f\|_2^2 + \delta^2\frac{\|f\|_{\mcA}^2}{B}
\end{equation}
Thus overall, we have:
\begin{equation}\label{eqn:reg-pop-emp}
    \forall f\in \mcF: \left|\|f\|_{n,2}^2 - \|f\|_2^2 \right| \leq \frac{1}{2} \|f\|_2^2 + \delta^2 \max\left\{1, \frac{\|f\|_{\mcA}^2}{B}\right\}
\end{equation}
Thus we have that w.p. $1-\zeta$: 
\begin{align}
    \forall f\in \mcF: \lambda \|f\|_{\mcA}^2 + \|f\|_{2,n}^2 \geq~& \lambda \|f\|_{\mcA}^2 + \frac{1}{2}\|f\|_{2}^2 - \delta^2 \max\left\{1, \frac{\|f\|_{\mcA}^2}{B}\right\}\\
    \geq~& \left(\lambda - \frac{\delta^2}{B}\right)\|f\|_{\mcA}^2 + \frac{1}{2}\|f\|_{2}^2 - \delta^2
\end{align}
Assuming that $\lambda \geq \frac{2\delta^2}{B}$, we have that, the latter is at least:
\begin{equation}
    \forall f\in \mcF: \lambda \|f\|_{\mcA}^2 + \|f\|_{2,n}^2 \geq \frac{\lambda}{2} \|f\|_{\mcA}^2 + \frac{1}{2}\|f\|_{2}^2 - \delta^2
\end{equation}


\paragraph{Upper bounding centered empirical sup-loss.} We now argue that the centered empirical sup-loss: 
$$\sup_{f \in \mcF} (\Psi_n(\hat{a}, f) - \Psi_n(a_*, f)) = \sup_{f \in \mcF} \E_n[(a_*(X)-\hat{a}(X))\, f(X)]$$ 
is small. By the definition of $\hat{a}$:
\begin{equation}\label{eqn:reg-optimality}
\sup_{f\in \mcF} \Psi_n^{\lambda}(\hat{a}, f) \leq \sup_{f\in \mcF} \Psi_n^{\lambda}(a_*, f) + \mu \left(\|a_*\|_{\mcA}^2 - \|\hat{a}\|_{\mcA}^2\right)
\end{equation}

By Lemma~7 of \cite{Foster2019}, the fact that $m(Z; f) - a_*(X) f(X)$ is $2$-Lipschitz with respect to the vector $(m(Z;f), f(z))$ (since $a_*(X)\in [-1, 1]$) and by our choice of $\delta:=\delta_n + c_0 \sqrt{\frac{\log(c_1/\zeta)}{n}}$, where $\delta_n$ is an upper bound on the critical radius of $\mcF_{B}$ and $m \circ \mcF_B$, w.p. $1-\zeta$:
\begin{align}
 \forall f\in \mcF_{B}: \left|\Psi_n(a_*, f) - \Psi(a_*, f)\right| \leq O\left(\delta \left(\|f\|_2 + \sqrt{\E[m(Z;f)^2]}\right) + \delta^2\right)
 =O\left(\delta\, M\, \|f\|_2 + \delta^2\right)
\end{align}
where we have invoked Assumption~\ref{ass:strong-smooth}. Thus, if $\|f\|_{\mcA} \geq \sqrt{B}$, we can apply the latter inequality for the function $f \sqrt{B}/\|f\|_{\mcA}$, which falls in $\mcF_{B}$, and then multiply both sides by $\|f\|_{\mcA}/\sqrt{B}$ (invoking the linearity of the operator $\Psi_n(a, f)$ with respect to $f$) to get:
\begin{align}\label{eqn:reg-concentration}
    \forall f \in \mcF: \left|\Psi_n(a_*, f) - \Psi(a_*, f)\right| \leq O\left(\delta\, M\, \|f\|_2 + \delta^2 \max\left\{1, \frac{\|f\|_{\mcA}}{\sqrt{B}}\right\}\right) 
\end{align}

By Equations~\eqref{eqn:reg-optimality} and \eqref{eqn:reg-concentration}, we have that w.p. $1-2\zeta$, for some universal constant $C$:
\begin{align}
   \sup_{f\in \mcF} \Psi_n^{\lambda}(a_*, f)
    =~& \sup_{f\in \mcF} \left(\Psi_n(a_*, f) - \|f\|_{2,n}^2 - \lambda \|f\|_{\mcA}^2\right)\\
    \leq~& \sup_{f\in \mcF} \left(\Psi(a_*, f) + C \delta^2 + \frac{C\delta^2}{\sqrt{B}}\|f\|_{\mcA} + C M \delta \|f\|_2 - \|f\|_{2,n}^2 - \lambda \|f\|_{\mcA}^2\right)\\
    \leq~& \sup_{f\in \mcF} \left(\Psi(a_*, f) + C \delta^2 + \frac{C\delta^2}{\sqrt{B}}\|f\|_{\mcA}  + C M\delta \|f\|_2 - \frac{1}{2} \|f\|_2^2 - \frac{\lambda}{2} \|f\|_{\mcA}^2 + \delta^2\right)\\
    \leq~& \sup_{f\in \mcF} \Psi^{\lambda/2}(a_*, f) + O\left(\delta^2\right)
    + \sup_{f\in \mcF} \left( \frac{C\delta^2}{\sqrt{B}}\|f\|_{\mcA} - \frac{\lambda}{4}\|f\|_{\mcA}^2\right) + \sup_{f\in \mcF} \left(C M\delta \|f\|_2 - \frac{1}{4}\|f\|_{2}^2\right)
\end{align}
Moreover, observe that for any norm $\|\cdot\|$ and any constants $a,b>0$:
\begin{align}
    \sup_{f\in \mcF} \left(a\|f\| - b \|f\|^2\right) \leq \frac{a^2}{4b}
\end{align}
Thus if we assume that $\lambda\geq 2\delta^2/B$, we have:
\begin{align}
\sup_{f\in \mcF} \left( \frac{C\delta^2}{\sqrt{B}}\|f\|_{\mcA} - \frac{\lambda}{4}\|f\|_{\mcA}^2\right) \leq~& \frac{C^2 \delta^4}{B \lambda} \leq \frac{C^2}{2} \delta^2\\
    \sup_{f\in \mcF} \left(C M\delta \|f\|_2 - \frac{1}{4}\|f\|_{2}^2\right) \leq~& C^2 M^2 \delta^2
\end{align}
Thus we have:
\begin{align}
    \sup_{f\in \mcF} \Psi_n^{\lambda}(a_*, f)\leq \sup_{f\in \mcF} \Psi^{\lambda/2}(a_*, f) + O\left(M^2\, \delta^2\right)
\end{align}
Moreover:
\begin{align}
\sup_{f\in \mcF} \Psi_n^{\lambda}(\hat{a}, f) =~& \sup_{f \in \mcF} \left(\Psi_n(\hat{a}, f) - \Psi_n(a_*, f) + \Psi_n(a_*, f) - \|f\|_{2,n}^2 - \lambda \|f\|_{\mcA}^2\right)\\ 
\geq~& \sup_{f \in \mcF} \left(\Psi_n(\hat{a}, f) - \Psi_n(a_*, f) - 2 \|f\|_{2,n}^2 - 2\, \lambda \|f\|_{\mcA}^2\right)  + \inf_{f\in \mcF} \left(\Psi_n(a_*, f) + \|f\|_{2,n}^2 + \lambda \|f\|_{\mcA}^2\right)
\end{align}
Observe that since $\Psi_n(a, f)$ is a linear operator of $f$ and $\mcF$ is a symmetric class, we have:
\begin{align}
    \inf_{f\in \mcF} \left(\Psi_n(a_*, f) + \|f\|_{2,n}^2 + \lambda \|f\|_{\mcA}^2\right) =~& \inf_{f\in \mcF} \left(\Psi_n(a_*, -f) + \|f\|_{2,n}^2 + \lambda \|f\|_{\mcA}^2\right)\\
    =~& \inf_{f\in \mcF} \left(- \Psi_n(a_*, f) + \|f\|_{2,n}^2 + \lambda \|f\|_{\mcA}^2\right)\\
    =~& - \sup_{f\in \mcF} \left(\Psi_n(a_*, f) - \|f\|_{2,n}^2 - \lambda \|f\|_{\mcA}^2\right) = -\sup_{f\in \mcF} \Psi_n^{\lambda}(a_*, f)
\end{align}
Combining this with Equation~\eqref{eqn:reg-optimality} yields:
\begin{align}
    \sup_{f \in \mcF} \left(\Psi_n(\hat{a}, f) - \Psi_n(a_*, f) - \|f\|_{2,n}^2 - \lambda \|f\|_{\mcA}^2\right) \leq~& 2\, \sup_{f\in \mcF} \Psi_n^{\lambda}(a_*, f) + \mu \left(\|a_*\|_{\mcA}^2 - \|\hat{a}\|_{\mcA}^2\right)\\
    \leq~& 2\,\sup_{f\in \mcF} \Psi^{\lambda/2}(a_*, f) + \mu \left(\|a_*\|_{\mcA}^2 - \|\hat{a}\|_{\mcA}^2\right) + O\left(M^2\, \delta^2\right)
\end{align}

\paragraph{Lower bounding centered empirical sup-loss.} First observe that:
\begin{equation}
    \Psi_n(a, f) - \Psi_n(a_*, f) = \E_n[(a_*(X)-a(X)) f(X)] 
\end{equation}
Let $\Delta=a_* - \hat{a}$. Suppose that $\|\Delta\|_2\geq \delta$ and let $r = \frac{\delta}{2\|\Delta\|_2}\in [0, 1/2]$. Then observe that since $\Delta\in \mcF$ and $\mcF$ is star-convex, we also have that $r \Delta\in \mcF$. Thus
\begin{align}
    \sup_{f \in \mcF} \left(\Psi_n(\hat{a}, f) - \Psi_n(a_*, f) - \|f\|_{2,n}^2 - \lambda \|f\|_{\mcA}^2\right) \geq~& 
    \Psi_n(\hat{a}, r\Delta) - \Psi_n(a_*, r\Delta) - r^2 \|\Delta\|_{2,n}^2 - \lambda r^2 \|\Delta\|_{\mcA}^2\\
    =~& r \E_n\left[(a_*(X) - \hat{a}(X))^2\right] - r^2 \|\Delta\|_{2,n}^2 - \lambda r^2 \|\Delta\|_{\mcA}^2\\
    =~& r \|\Delta\|_{2,n}^2 - r^2 \|\Delta\|_{2,n}^2 - \lambda r^2 \|\Delta\|_{\mcA}^2\\
    \geq~& r \|\Delta\|_{2,n}^2 - r^2 \|\Delta\|_{2,n}^2 - \lambda \|\Delta\|_{\mcA}^2
\end{align}

Moreover, since $\delta_n$ upper bounds the critical radius of $\mcF_{B}$ and by Equation~\eqref{eqn:reg-pop-emp}:
\begin{align}
    r^2 \|\Delta\|_{2,n}^2
    \leq~& r^2 \left(2\|\Delta\|_2^2 + \delta^2 + \delta^2 \frac{\|\Delta\|_{\mcA}^2}{B}\right)\\
    \leq~& 2\delta^2 + \delta^2 \frac{\|\Delta\|_{\mcA}^2}{B} \leq 2\delta^2 + \lambda \|\Delta\|_{\mcA}^2
\end{align}
Thus we get:
\begin{align}
    \sup_{f \in \mcF} \left(\Psi_n(\hat{a}, f) - \Psi_n(a_*, f) - \|f\|_{2,n}^2 - \lambda \|f\|_{\mcA}^2\right) \geq~& r \|\Delta\|_{2,n}^2 - 2\delta^2 - 2\lambda \|\Delta\|_{\mcA}^2
\end{align}
Furthermore, again, since $\delta_n$ upper bounds the critical radius of $\mcF_{B}$ and by Equation~\eqref{eqn:reg-pop-emp}:
\begin{align}
    \|\Delta\|_{2,n}^2 \geq \frac{1}{2} \|\Delta\|_2^2 - \frac{\delta^2}{2B}\|\Delta\|_{\mcA}^2 - \delta^2 \geq \frac{1}{2} \|\Delta\|_2^2 - \lambda\|\Delta\|_{\mcA}^2 - \delta^2
\end{align}
Thus we have:
\begin{align}
    \sup_{f \in \mcF} \left(\Psi_n(\hat{a}, f) - \Psi_n(a_*, f) - \|f\|_{2,n}^2 - \lambda \|f\|_{\mcA}^2\right) \geq~& \frac{r}{2} \|\Delta\|_{2}^2 - 3\delta^2 - 3\lambda \|\Delta\|_{\mcA}^2\\
    \geq~& \frac{\delta}{4} \|\Delta\|_2  - 3\delta^2 - 3\lambda \|\Delta\|_{\mcA}^2
\end{align}


\paragraph{Combining upper and lower bound.} Combining the upper and lower bound on the centered population sup-loss we get that w.p. $1-3\zeta$: either $\|\Delta\|_2\leq \delta$ or:
\begin{align}
    \frac{\delta}{4} \|\Delta\|_2 \leq~& O\left(M^2\, \delta^2\right) + 2\,\sup_{f\in \mcF} \Psi^{\lambda/2}(a_*, f) + 3\lambda \|\Delta\|_{\mcA}^2 + \mu \left(\|a_*\|_{\mcA}^2 - \|\hat{a}\|_{\mcA}^2\right)
\end{align}
We now control the last part. Since $\mu \geq 6\lambda$:
\begin{align}
    3\lambda \|\Delta\|_{\mcA}^2 + \mu \left(\|a_*\|_{\mcA}^2 - \|\hat{a}\|_{\mcA}^2\right) \leq~&  6\lambda \left(\|a_*\|_{\mcA}^2 + \|\hat{a}\|_{\mcA}^2\right) + \mu \left(\|a_*\|_{\mcA}^2 - \|\hat{a}\|_{\mcA}^2\right) \leq 2 \mu \|a_*\|_{\mcA}^2
\end{align}
We can then conclude that:
\begin{equation}
    \frac{\delta}{4} \|\Delta\|_2 \leq O\left(M^2\, \delta^2\right) + 2\,\sup_{f\in \mcF} \Psi^{\lambda/2}(a_*, f) + 2 \mu \|a_*\|_{\mcA}^2
\end{equation}
Dividing over by $\delta/4$, we get:
\begin{equation}
     \|\Delta\|_2 \leq O\left(M^2\, \delta\right) + \frac{8}{\delta}\,\sup_{f\in \mcF} \Psi^{\lambda/2}(a_*, f) + 8 \frac{\mu}{\delta} \|a_*\|_{\mcA}^2
\end{equation}
Thus either $\|\Delta\|_2\leq \delta$ or the latter inequality holds. Thus in any case the latter inequality holds.

\paragraph{Upper bounding population sup-loss at minimum.} Observe that by the definition of the Riesz representer:
\begin{align}
    \sup_{f\in \mcF} \Psi^{\lambda/2}(a_*, f) =~& \sup_{f\in \mcF} \E[ (a_0(X)-a_*(X))\, f(z) ] - \frac{1}{4} \|f\|_2^2 - \frac{\lambda}{4}\|f\|_{\mcA}^2\\
    \leq~& \sup_{f\in \mcF} \E[ (a_0(X) - a_*(X))\, f(z) ] - \frac{1}{4} \|f\|_{2}^2
    = \|a_0 - a_*\|_2^2
\end{align}

\paragraph{Concluding.} Concluding we get that w.p. $1-3\zeta$:
\begin{equation}
    \|\hat{a}-a_*\|_2 \leq O\left(M^2\, \delta\right) + \frac{8}{\delta}\, \|a_*-a_0\|_2^2 + 8 \frac{\mu}{\delta} \|a_*\|_{\mcA}^2
\end{equation}
By a trinagle inequality we get:
\begin{equation}
    \|\hat{a}-a_0\|_2 \leq O\left(M^2\, \delta\right) + \frac{8}{\delta}\, \|a_*-a_0\|_2^2 + \|a_* - a_0\|_2 + 8 \frac{\mu}{\delta} \|a_*\|_{\mcA}^2
\end{equation}

Choosing $a_* = \argmin_{a\in \mcA} \|a-a_0\|_2$ and using the fact that $\delta \geq \epsilon_n$, we get:
\begin{equation}
    \|\hat{a}-a_0\|_2 \leq O\left(M^2 \delta + \|a_*-a_0\|_2 + \frac{\mu}{\delta} \|a_*\|_{\mcA}^2\right) \leq O\left(M^2 \delta + \frac{\mu}{\delta} \|a_*\|_{\mcA}^2\right)
\end{equation}
\end{proof}


\subsection{Proof of \Cref{thm:reg-main-error-2}}

\begin{proof}
By the definition of $\hat{a}$:
\begin{equation}
    0\leq \sup_{f} \Psi_n(\hat{a}, f) \leq \sup_{f} \Psi_n(a_0, f) + \lambda \left(\|a_0\|_{\mcA} - \|\hat{a}\|_{\mcA}\right)
\end{equation}
Let
\[
\delta_{n, \zeta}=\max_{i}\left(\mcR(\mcF^i) + \mcR(m\circ \mcF^i)\right) + c_0 \sqrt{\frac{\log(c_1/\zeta)}{n}}
\]
for some universal constants $c_0,c_1$. By Theorem~26.5 and 26.9 of \cite{shalev2014understanding}, and since $\mcF^i$ is a symmetric class and since $\|a_0\|_{\infty} \leq 1$, w.p. $1-\zeta$:
\begin{equation}
    \forall f\in \mcF^i: \left|\Psi_n(a_0, f) - \Psi(a_0, f)\right| \leq \delta_{n,\zeta}
\end{equation}
Since $\Psi(a_0, f)=0$ for all $f\in \mcF$, we have that, w.p. $1-\zeta$:
\begin{equation}
    \|\hat{a}\|_{\mcA} \leq \|a_0\|_{\mcA} + \delta_{n,\zeta}/\lambda 
\end{equation}
Let $B_{n,\lambda,\zeta} = (\|a_0\|_{\mcH} + \delta_{n,\zeta}/\lambda)^2$, $\mcA_B\cdot \mcF^i := \{a\cdot f: a\in \mcA_B, f\in \mcF^i\}$ and
\[
\epsilon_{n,\lambda, \zeta}=\max_{i}\left(\mcR(\mcA_{B_{n,\lambda,\zeta}}\cdot \mcF^i) + \mcR(m\circ \mcF^i)\right) + c_0 \sqrt{\frac{\log(c_1/\zeta)}{n}}
\]
for some universal constants $c_0,c_1$, then again by Theorem~26.5 and 26.9 of \cite{shalev2014understanding},
\begin{equation}
    \forall a\in \mcA_{B_{n,\lambda,\zeta}}, f\in \mcF_U^i \left|\Psi_n(a, f) - \Psi(a, f)\right| \leq \epsilon_{n,\lambda, \zeta}
\end{equation}
By a union bound over the $d$ function classes composing $\mcF$, we have that w.p. $1-2\zeta$:
\begin{equation}
    \sup_{f\in \mcF} \Psi_n(a_0, f) \leq \sup_{f\in \mcF} \Psi(a_0, f) + \delta_{n,\zeta/d} = \delta_{n,\zeta/d}
\end{equation}
and
\begin{equation}
    \sup_{f\in \mcF} \Psi_n(\hat{a}, f) \geq \sup_{f\in \mcF} \Psi(\hat{a}, f) - \epsilon_{n,\lambda, \zeta/d}
\end{equation}
If $\|\hat{a}-a_0\|_2\leq \delta_{n,\zeta}$, then the theorem follows immediately. Thus we consider the case when $\|\hat{a}-a_0\|_2\geq \delta_{n,\zeta}$. Since, by assumption, for any $a\in \mcA_{B}$ with $\|a-a_0\|\geq \delta_{n,\zeta}$ it holds that $\frac{a_0-a}{\|a_0-a\|_2}\in \spanF_{\kappa}(\mcF)$, we have $\frac{a_0 -\hat{a}}{\|a_0 - \hat{a}\|_2}=\sum_{i=1}^p w_i f_i$, with $p<\infty$, $\|w\|_1\leq \kappa$ and $f_i\in \mcF$. Thus:
\begin{align}
    \sup_{f\in \mcF} \Psi(\hat{a}, f) \geq~& \frac{1}{\kappa} \sum_{i=1}^p w_i \Psi(\hat{a}, f_i) = \frac{1}{\kappa} \Psi\left(\hat{a}, \sum_i w_i f_i\right)\\
    =~& \frac{1}{\kappa} \frac{1}{\|\hat{a}-a_0\|_2}\Psi(\hat{a}, a_0 - \hat{a})\\
    =~& \frac{1}{\kappa} \frac{1}{\|\hat{a}-a_0\|_2}\E[(a_0(X) - \hat{a}(X))^2]\\
    =~& \frac{1}{\kappa} \|\hat{a}-a_0\|_2
\end{align}
Combining all the above we have, w.p. $1-2\zeta$:
\begin{equation}
    \|\hat{a}-a_0\|_2 \leq \kappa\, \left(\epsilon_{n, \lambda, \zeta/d} + \delta_{n,\zeta/d} + \lambda \left(\|a_0\|_{\mcA} - \|\hat{a}\|_{\mcA}\right)\right)
\end{equation}
Moreover, since functions in $\mcA$ and $\mcF$ are bounded in $[-1,1]$, we have that the function $a\cdot f$ is $1$-Lipschitz with respect to the vector of functions $(a, f)$. Thus we can apply a vector version of the contraction inequality \cite{maurer2016vector} to get that:
\begin{equation}
\mcR(\mcA_{B_{n,\lambda, z}}\cdot \mcF^i) \leq 2\, \left(\mcR(\mcA_{B_{n,\lambda, z}}) + \mcR(\mcF^i)\right)
\end{equation}
Finally, we have that since $\mcA$ is star-convex:
\begin{equation}
    \mcR(\mcA_{B_{n,\lambda, z}}) \leq \sqrt{B_{n,\lambda, z}}\,\mcR(\mcA_1)
\end{equation}
Leading to the final bound of:
\begin{multline}
    \|\hat{a}-a_0\|_2 \leq \kappa \left( 2\left(\|a_0\|_{\mcA} + \delta_{n,\zeta}/\lambda\right) \mcR(\mcA_1) + 2\, \max_{i=1}^d \left(\mcR(\mcF^i) + \mcR(m\circ \mcF^i)\right) \right)\\ + \kappa \left(c_0\sqrt{\frac{\log(c_1\, d/\zeta)}{n}} + \lambda \left(\|a_0\|_{\mcA}-\|\hat{a}\|_{\mcA}\right)\right)
\end{multline}
Since $\lambda \geq \delta_{n,\zeta}$, we get the result.
\end{proof}

\subsection{Proof of \Cref{cor:sparse-linear-reg-ell1}}

\begin{proof}
Consider any $\hat{a}=\ldot{\hat{\theta}}{\cdot}\in \mcA_{B_{n,\lambda,\zeta}}$ and let $\nu=\hat{\theta} - \theta_0$, then:
\begin{align}
    \delta_{n,\zeta}/\lambda + \|\theta_0\|_1 \geq \|\hat{\theta}\|_1 =\|\theta_0 + \nu\|_1 = \|\theta_0 + \nu_S\|_1+\|\nu_{S^c}\|_1 \geq \|\theta_0\|_1 - \|\nu_S\|_1 + \|\nu_{S^c}\|_1
\end{align}
Thus:
\begin{equation}
    \|\nu_{S^c}\|_1\leq \|\nu_S\|_1 + \delta_{n,\zeta}/\lambda
\end{equation}
and $\nu$ lies in the restricted cone for which the restricted eigenvalue of $V$ holds. Moreover, since $|S|=s$:
\begin{equation}
    \|\nu\|_1 \leq 2 \|\nu_S\|_1 + \delta_{n,\zeta}/\lambda \leq 2\sqrt{s} \|\nu_S\|_2  + \delta_{n,\zeta}/\lambda \leq 2\sqrt{s}\|\nu\|_2  + \delta_{n,\zeta}/\lambda \leq 2 \sqrt{\frac{s}{\gamma} \nu^\top  V \nu}  + \delta_{n,\zeta}/\lambda 
\end{equation}
Moreover, observe that: 
\begin{equation}
    \|\hat{a}-a_0\|_2 = \sqrt{\E[ \ldot{\nu}{x}^2 ]} = \sqrt{\nu^\top  V \nu} 
\end{equation}
Thus we have:
\begin{equation}
    \frac{\hat{a}(x)-a_0(x)}{\|\hat{a}-a_0\|_2} = \sum_{i=1}^p \frac{\nu_i}{\sqrt{\nu^\top V\nu}} x_i 
\end{equation}
Thus for any $\hat{a}\in \mcA_{B_{n,\lambda,\zeta}}$, we can write $\frac{\hat{a}-a_0}{\|\hat{a}-a_0\|_2}$ as $\sum_{i=1}^p w_i f_i$, with $f_i\in \mcF$ and:
\begin{equation}
    \|w\|_1 = \frac{\|\nu\|_1}{\sqrt{\nu^\top V \nu}} \leq 2\sqrt{\frac{s}{\gamma}} + \frac{\delta_{n,\zeta}}{\lambda} \frac{1}{\|\hat{a}-a_0\|_2}.
\end{equation}
Thus: $\frac{\hat{a}-a_0}{\|\hat{a}-a_0\|_2} \in \spanF_{\kappa}(\mcF)$ for $\kappa=2\sqrt{\frac{s}{\gamma}} + \frac{\delta_{n,\zeta}}{\lambda} \frac{1}{\|\hat{a}-a_0\|_2}$.

Moreover, observe that by the triangle inequality:
\begin{equation}
    \|a_0\|_{\mcA} - \|\hat{a}\|_{\mcA} = \|\theta_0\|_1 - \|\hat{\theta}\|_1 \leq \|\theta_0-\hat{\theta}\|_1 = \|\nu\|_1 \leq 2 \sqrt{\frac{s}{\gamma} \nu^\top  V \nu}  + \delta_{n,\zeta}/\lambda 
\end{equation}
Moreover, by standard results on the Rademacher complexity of linear function classes (see e.g. Lemma~26.11 of \cite{shalev2014understanding}), we have $\mcR(\mcA_B)\leq B\sqrt{\frac{2\log(2\, p)}{n}}\max_{x\in \mcX} \|x\|_{\infty}$ and $\mcR(\mcF^i), \mcR(m\circ \mcF^i)\leq \sqrt{\frac{2\log(2)}{n}}\max_{x\in \mcX} \|x\|_{\infty}$ (the latter via the fact that each $\mcF^i$; and therefore also $m\circ \mcF^i$; contains only two elements and invoking Masart's lemma). Thus invoking \Cref{thm:reg-main-error-2}:
\begin{align}
    \|\hat{a}-a_0\|_2 \leq~& \left(2\sqrt{\frac{s}{\gamma}} + \frac{\delta_{n,\zeta}}{\lambda} \frac{1}{\|\hat{a}-a_0\|_2}\right)\cdot \left(2 (\|\theta_0\|_{1}+1) \sqrt{\frac{\log(2p)}{n}} + \delta_{n,\zeta} + \lambda \sqrt{\frac{s}{\gamma}} \|\hat{a}-a_0\|_2\right)
\end{align} 
The right hand side is upper bounded by the sum of the following four terms:
\begin{align}
    Q_1 :=~& 2\sqrt{\frac{s}{\gamma}} \left(2(\|\theta_0\|_1+1) \sqrt{\frac{\log(2p)}{n}} + \delta_{n,\zeta}\right)\\
    Q_2 :=~& \left(\frac{\delta_{n,\zeta}}{\lambda} \frac{1}{\|\hat{a}-a_0\|_2}\right)\left(2 (\|\theta_0\|_1+1) \sqrt{\frac{\log(2p)}{n}} + \delta_{n,\zeta} \right)\\
    Q_3 :=~& 2 \lambda \frac{s}{\gamma} \|\hat{a}-a_0\|_2\\
    Q_4 :=~& \delta_{n,\zeta} \sqrt{\frac{s}{\gamma}}
\end{align}
If $\|\hat{a}-a_0\|_2 \geq \sqrt{\frac{s}{\gamma}} \delta_{n,\zeta}$ and setting $\lambda \leq \frac{\gamma}{8s}$, yields:
\begin{align}
    Q_2 \leq~& 8 \frac{1}{\lambda}\sqrt{\frac{\gamma}{s}}\left(2 (\|\theta_0\|_1+1) \sqrt{\frac{\log(2p)}{n}} + \delta_{n,\zeta} \right)\\
    Q_3 \leq~& \frac{1}{4} \|\hat{a}-a_0\|_2
\end{align}
Thus bringing $Q_3$ on the left-hand-side and dividing by $3/4$, we have:
\begin{equation}
    \|\hat{a}-a_0\|_2 \leq \frac{4}{3} (Q_1 + Q_2 + Q_4) = \frac{4}{3}\max\left\{\sqrt{\frac{s}{\gamma}}, \frac{1}{\lambda} \sqrt{\frac{\gamma}{s}}\right\} \left(20\, (\|\theta_0\|_1+1) \sqrt{\frac{\log(2p)}{n}} + 11 \delta_{n,\zeta}\right)
\end{equation}
On the other hand if $\|\hat{a}-a_0\|_2\leq \sqrt{\frac{s}{\gamma}} \delta_{n,\zeta}$, then the latter inequality trivially holds. Thus it always holds.
\end{proof}