\section{$k_1 > 1$}\label{sec:Case1}
In the present section we classify all the changemaker C-type lattices that have 
\[
x_0=e_0 \pm e_{k_1} \pm e_{k_2} \pm e_{k_3},
\]
where $k_1>1$. Using Lemma~\ref{Lem:X0Odd}, we know that
\begin{equation}\label{eq:v1}
v_1=2e_0 - e_1,
\end{equation}
and therefore, $\sigma_1 =2$ and $|v_1|=5$. We remind the reader that, by Lemma~\ref{lem:tightvector}, $v_1$ is the only tight vector in the C-type lattices that concern us in this section. We also note that 
\begin{equation}\label{eq:0inVk1}
0\in\supp(v_{k_1})
\end{equation}
 by Lemma~\ref{Lem:X0Odd}.
Compared to Sections~\ref{sec:Case2}~and~\ref{sec:k1k21}, it will take longer to determine the initial segment $(\sigma_0, \cdots, \sigma_{k_3})$ of $\sigma$. We start by specifying the positive integer $k_1$. 


\begin{lemma}\label{lem:k1>1,v2+t}
		The segment $(\sigma_0, \cdots \sigma_{k_1})$ is either $(1,2,3)$ or $(1,2,2,3)$. In particular, $k_1=2$ or $3$, and $\sigma_{k_1}=3$. 
\end{lemma}

\begin{proof}
Using Lemma~\ref{lem:tightvector}, we get that $v_2$ is either $e_0+e_1-e_2$ or $e_1-e_2$. In the former case, using Lemma~\ref{Lem:X0Odd}, we get that $k_1=2$, and so $\sigma_{k_1}=3$. 

Now suppose that $v_2=e_1-e_2$. More generally, suppose that there exists $t\ge 1$ such that $(\sigma_0, \sigma_1, \cdots, \sigma_{t+1})=(1,2,2^{[t]})$, and that $|v_{t+2}|>2$. We will show that $t=1$, $k_1=3$, and that $\sigma_{t+2}$ (or simply $\sigma_3$) is $3$. 

Set $j=\min\supp(v_{t+2})$. We argue that $j=0$. (Note that, by Lemma~\ref{gappy3}, none of $1,2, \cdots, t$ is a gappy index for $v_{t+2}$.) If $1<j<t+1$, there will be a claw on $v_j, v_{j-1}, v_{t+2}, v_{j+1}$. If $j=1$, then $\braket{v_{t+2}}{v_1}=-1$ and $v_{t+2}$ will be orthogonal to $v_2$. Then $k_1>t+2$ by \eqref{eq:0inVk1}.
There will be a claw on $v_1, x_0, v_{t+2}, v_2$, unless $[v_{t+2}]\pitchfork [v_1]$, $|[v_1\cap v_{t+2}]|=|v_{t+2}|=3$, and $\epsilon_{t+2}=-\epsilon_1$. Thus $v_1+v_{t+2}$ is the sum of two distant intervals and so is reducible. Since $|v_{t+2}|=3$, $v_{t+2}=e_1+e_{t+1}-e_{t+2}$, and so $v_1+v_{t+2}$ is irreducible by Lemma~\ref{lem:SumIrr}, a contradiction. That is, $j=0$, and that, 
\begin{equation}\label{vt+2}
v_{t+2}=e_0+e_{i}+e_{i+1} + \cdots + e_{t+1}-e_{t+2},
\end{equation}
with $i\ge 1$. 

Since $0\in \supp^+(v_{t+2})$, using Lemma~\ref{Lem:X0Odd}, we get that $k_1=t+2$. Furthermore, we claim that 
$x_0=e_0+e_{t+2}+e_{k_2}-e_{k_3}$. See Proposition~\ref{x0}. If $x_0=e_0-e_{t+2}-e_{k_2}+e_{k_3}$, then $\braket{v_{t+2}}{x_0}=2$. 
% Since $|v_2|=2$ and $\braket{v_1}{v_2}=-1$, it cannot be the case that $[v_2]\pitchfork [v_1]$ (as otherwise $\braket{v_1}{v_2}=0$). Moreover, since $v_2$ is orthogonal to $x_0$, it must be that either $[v_1]$ and $[v_2]$ share the right endpoint of $[v_1]$, or $[v_2]\dagger[v_1]$ and the left endpoint of $[v_2]$ is to the right of the right endpoint of $[v_1]$. In either of these cases, since $[v_{t+2}]$ is an interval of high norm, it cannot be both $[v_{t+2}]\pitchfork [v_1]$ and $\braket{v_2}{v_{t+2}}$. 
Observe that $\braket{v_{t+2}}{v_1}=1$ or $2$ depending on whether or not $i=1$ in~\eqref{vt+2}; in particular, $\braket{v_{t+2}}{v_1}>0$. Since $|v_{t+2}\cap v_1|=|v_{t+2}|\ge 3$ and $\delta([v_1],[v_{t+2}])\le 3$, using Lemma~\ref{intervalproduct}, it must be that $\epsilon_1 = \epsilon_{t+2}$. Since $\braket{v_1}{x_0}=\braket{v_{t+2}}{x_0}=2$, $[v_1]$ and $[v_{t+2}]$ share their left endpoint, and $\delta([v_{t+2}], [v_1])=1$. Moreover, we must have $|v_{t+2}|=3$ (as otherwise $\braket{v_{t+2}}{v_1}>2$). That is, $v_{t+2}=e_0+e_{t+1}-e_{t+2}$. We have $\braket{v_2}{v_1}=-1$ and $\braket{v_2}{x_0}=0$, so $[v_2]$ abuts the right end of $[v_1]$.
Since also $v_{t+2}\sim v_{t+1}$, $|v_i|=2$ for $i\in \{ 2, \cdots, t+1\}$,
\[
v_2\sim v_3\sim\cdots\sim v_{t+1},
\]
 the interval $[v_1]$ is a subset of the union of the $[v_j]$ for $j\in \{ 2, \cdots, t+2\}$, which in turn implies that $|v_1|=|v_{t+2}|=3$, a contradiction. This shows that 
\[
x_0=e_0+e_{t+2}+e_{k_2}-e_{k_3}.
\]

We now argue that $1\not \in \supp(v_{t+2})$. Suppose for contradiction that $1\in \supp(v_{t+2})$. Using (\ref{vt+2}), we get
 that $|v_{t+2}|\ge 4$, $\braket{v_1}{v_{t+2}}=1$ and $\braket{v_2}{v_{t+2}}=0$. To avoid a claw on $v_1, x_0, v_{t+2}, v_2$, we must have $[v_{t+2}]\pitchfork [v_1]$. This implies that $\delta([v_1], [v_{t+2}])=2$. Using Lemma~\ref{intervalproduct} and that $|v_{t+2}|\ge 4$, we see that $|\braket{v_1}{v_{t+2}}|\ge 2$, a contradiction. That is, in~\eqref{vt+2}, we must have $i>1$. 

We claim that $i=2$. If $2<i<t+1$, there will be a claw on $v_i, v_{i-1}, v_{t+2}, v_{i+1}$. If $i=t+1$ (and $i>2$), to avoid a claw on $v_1, x_0, v_{t+2}, v_2$, it must be that $[v_{t+2}]\pitchfork [v_1]$, and so $\delta([v_{t+2}], [v_1])=2$. To get $\braket{v_{t+2}}{v_1}=2$, however, it must be $|v_{t+2}|=4$ which contradicts $i=t+1$. Therefore, in~\eqref{vt+2}, we have $i=2$. In particular, $v_2\sim v_{t+2}$.

Finally, we argue that $t=1$. If $t>1$, we must have $v_1\sim v_{t+2}$ as otherwise we get a claw $(v_2, v_1, v_{t+2}, v_3)$. That is, $[v_{t+2}]$ abuts $[v_1]$. Therefore, to fulfill $\braket{v_{t+2}}{v_1}=2$, $[v_{t+2}]\prec[v_1]$, and that $|v_{t+2}|=3$, which contradicts $t>1$ and (\ref{vt+2}). So $t=1$ as desired.
\end{proof}

As part of the proof of Lemma~\ref{lem:k1>1,v2+t}, we showed that $x_0 = e_0+e_{k_1}+e_{k_2}-e_{k_3}$ when $k_1=3$. Indeed, this is the case also when $k_1=2$.

\begin{lemma}\label{lem:k1>1, chi=2}
		Let $k_1>1$. Then $x_0 = e_0+e_{k_1}+e_{k_2}-e_{k_3}$.
\end{lemma}

\begin{proof}
We only need to show this for $k_1=2$. Suppose for contradiction $x_0 = e_0-e_{2}-e_{k_2}+e_{k_3}$ (see Proposition~\ref{x0}). Note that $v_2=e_0+e_1-e_2$, and therefore, $\braket{v_2}{x_0}=2=\braket{v_1}{x_0}$, and $\braket{v_2}{v_1}=1$. Since $|v_2|=3$, using Lemma~\ref{intervalproduct}, we see that $\epsilon_1=\epsilon_2$ and $\delta([v_1],[v_2])=2$. Since $\braket{[v_2]}{x_0}=\braket{[v_1]}{x_0}=\pm2$, $[v_1],[v_2]$ share their left end point, so we cannot have $\delta([v_1],[v_2])=2$, a contradiction.
\end{proof}

Now we proceed to determine the changemaker vectors. As in Section~\ref{sec:Case2}, we use the notation of~\eqref{Eq:Sj}~and~\eqref{Eq:S'j}. Also, we use the basis $S'$, defined in~\eqref{Eq:S'}, where $v_{k_3}$ is replaced by $x_0$.

\input{k1=2}
\input{k1=3}


