\section{K\"ulshammer's question (Proof of Theorem~\ref{thmKul})}
Let $d\geq 5$ be odd. Let $D_{2d}$ be the dihedral group of order $2d$. Let 
\begin{equation*}
\Gamma:=D_{2d}\times C_2 =\langle r, s, z\mid r^d=s^2=z^2=1, srs^{-1}=r^{-1}, [r,z]=[s,z]=1\rangle.
\end{equation*}
Let $\Gamma_2:=\langle s, z\rangle$ (a Sylow $2$-subgroup of $\Gamma$). Let $G$ be as in the hypothesis. Choose $a, b\in k^{*}$ with $b^d=1$ and $b\neq 1$. Let $n:=n_\alpha n_\gamma n_\delta$ and $t:=(\alpha+\gamma+\delta)^{\vee}(b)$. For each $a\in k$ define $\rho_a\in \textup{Hom}(\gamma, G)$ by
\begin{equation*}
\rho_a(r)=t, \; \rho_a(s)=n \epsilon_{12}(a), \; \rho_a(z)=\epsilon_{12}(1). 
\end{equation*}
An easy computation shows that this is well-defined. 
Let $u(\sqrt a)=\epsilon_{4}(\sqrt a)\epsilon_{11}(\sqrt a)$. Then $u(\sqrt a)\cdot n = n\epsilon_{12}(a)$ and $u(\sqrt a)\cdot \epsilon_{12}(1) = \epsilon_{12}(1)$. Thus $u(\sqrt a)\cdot (\rho_0\mid_{\Gamma_2})=\rho_a\mid_{\Gamma_2}$. So $\rho_a\mid_{\Gamma_2}$ are pairwise conjugate. 

Now suppose that $\rho_a$ is conjugate to $\rho_b$. Then there exists $g\in G$ such that $g\cdot \rho_a=\rho_b$. Since $\rho_a(r)=t$, we must have $g\in C_G(t)=TG_{12}$. So let $g=hm$ for some $h\in T$ and $m\in G_{12}$. Then we have
\begin{alignat*}{2}
hnh^{-1}(hm\epsilon_{12}(a)m^{-1}h^{-1})&= hnm\epsilon_{12}(a)m^{-1}h^{-1}\\
                                                                 &= hmn\epsilon_{12}(a)m^{-1}h^{-1}\\
                                                                 &= g\cdot \rho_{a}(s)\\
                                                                 &= \rho_b(s)\\
                                                                 &= n\epsilon_{12}(b).
\end{alignat*}
Note that $hnh^{-1}\in G_\alpha G_\gamma G_\delta$ and $hm\epsilon_{12}(a)m^{-1}h^{-1}\in G_{12}$. Since $[G_\alpha G_\gamma G_\delta, G_{12}]=1$, we have $G_\alpha G_\gamma G_\delta \cap G_{12}=1$. This implies $hnh^{-1}=n$. Now an easy computation shows $h\in G_{12}$. Thus $g=hm\in G_{12}$. Since $G_{12}$ is a simple group of type $A_1$, $(n\epsilon_{12}(a), \epsilon_{12}(1))$ cannot be $G_{12}$- conjugate to $(n\epsilon_{12}(b), \epsilon_{12}(1))$ if $a\neq b$. We are done.                                                                 
