\subsection{Proofs for Lemma \ref{gmm_ti}}\label{gmm1}
Before going to the proof of this theorem, we first state some basic definitions and useful lemmas. We define the balls of radius $8\sqrt{d\log K}$ around each $u_{i}^{*}$ and $u_{i}$ as
\%
\Omega_{i}^{*}:=\left\{ x \in \R^{d} \mid \|x-u_{i}^{*}\| \leq 8 \sqrt{d\log K}\right\}
\%
\%
\Omega_{i}:=\left\{ x \in \R^{d} \mid \|x-u_{i}\| \leq 8 \sqrt{d\log K}\right\}
\%
We denote the p.d.f of $\mathcal{N}\left(u_i, I_d\right)$ and $\mathcal{N}\left(u_i^{*}, I_d\right)$ by $P_{i}$ and $P_{i}^{*}$ respectively.

\begin{lemma} \label{initial_match}
If 
\%
d_{\mathrm{TV}}\left(p_{\mathbf{u}}(x), p_{\mathbf{u}^* }(x)\right) \leq \frac{1}{4K},
\%
then there exists a permutation of $\boldsymbol{u}$ such that $\|u_{i}^{*}-u_{i}\| \leq 16\sqrt{d\log{K}}$ holds for every $1\leq i \leq K$.
\end{lemma}

Before proving Lemma \ref{initial_match}, we first state a useful result of Gaussian norm concentration.
\begin{lemma} \label{norm_subGaussian}
Let $X \sim \mathcal{N}\left(0, I_d\right) $, then 
\%
\P (\|X\| \geq t) \leq 2\exp(-\frac{t^{2}}{16d}).
\%
\end{lemma}
\begin{proof}
This is a simple application of \cite{jin2019short} Lemma 1.3. Notice that $X$ is $1$-subGaussian, therefore taking $\sigma=\sqrt{d}$ in \cite{jin2019short} Lemma 1.3 yields what we want.
\end{proof}

\begin{proof}[Proof of Lemma \ref{initial_match}]
We prove by contradiction. If the statement is not true, since the separation satisfies $100\sqrt{d\log{K}} \geq 2 \cdot 16\sqrt{d\log{K}},$
there must exist a $u_{i}^{*}$ (W.L.O.G., denote it by $u_{1}^{*}$), such that $\|u_{1}^{*}-u_{j}\| > 16\sqrt{d\log{K}} $
for any $1 \leq j \leq K$.  Then 
\begin{align}
2 d_{\mathrm{TV}}\left(p_{\mathbf{u}}(x), p_{\mathbf{u}^* }(x)\right) 
&= \int_{\R^{d}} \bigg|\frac{1}{K}\sum_{i=1}^{K} P_{i}^{*}- \frac{1}{K}\sum_{i=1}^{K} P_{i}  \bigg| \mathrm{d}x \notag\\
& \geq \int_{\Omega_{1}^{*}} \bigg|\frac{1}{K}\sum_{i=1}^{K} P_{i}^{*}- \frac{1}{K}\sum_{i=1}^{K} P_{i}  \bigg| \mathrm{d}x \notag\\
& \geq \int_{\Omega_{1}^{*}} \frac{1}{K}\sum_{i=1}^{K} P_{i}^{*}\mathrm{d}x - \int_{\Omega_{1}^{*}} \frac{1}{K}\sum_{i=1}^{K} P_{i}\mathrm{d}x \notag\\
& \geq \int_{\Omega_{1}^{*}} \frac{1}{K} P_{1}^{*} \mathrm{d}x - \frac{1}{K}\sum_{i=1}^{K} \int_{\Omega_{1}^{*}}  P_{i}\mathrm{d}x \notag\\
& = \frac{1}{K} \P (\mathcal{N}\left(u_1^{*}, I_d\right) \in \Omega_{1}^{*}) - \frac{1}{K}\sum_{i=1}^{K} \P (\mathcal{N}\left(u_i, I_d\right) \in \Omega_{1}^{*})
\end{align}
Since $\|u_{1}^{*}-u_{i}\| > 16\sqrt{d\log{K}} $, therefore $\Omega_{1}^{*} \cap \Omega_{i} = \emptyset$, which implies (by Lemma \ref{norm_subGaussian})
\%
\P (\mathcal{N}\left(u_i, I_d\right) \in \Omega_{1}^{*}) \leq \P (\mathcal{N}\left(u_i, I_d\right) \in \Omega_{i}^{\mathbf{C}}) \leq 2\exp (-\frac{(8\sqrt{d\log K})^{2}}{16d}) = 2e^{-4\log K}
\%
Also, by Lemma \ref{norm_subGaussian},
\%
\P (\mathcal{N}\left(u_1^{*}, I_d\right) \in \Omega_{1}^{*}) \geq 1- 2\exp (-\frac{(8\sqrt{d\log K})^{2}}{16d}) = 1- 2e^{-4\log K}
\%
Therefore,
\begin{align}
2 d_{\mathrm{TV}}\left(p_{\mathbf{u}}(x), p_{\mathbf{u}^* }(x)\right)
& \geq \frac{1}{K} \P (\mathcal{N}\left(u_1^{*}, I_d\right) \in \Omega_{1}^{*}) - \frac{1}{K}\sum_{i=1}^{K} \P (\mathcal{N}\left(u_i, I_d\right) \in \Omega_{1}^{*}) \notag\\
& \geq \frac{1}{K} (1- 2e^{-4 \log K}) - \frac{1}{K}\sum_{i=1}^{K} 2e^{-4 \log K} \notag\\
& = \frac{1}{K} - (2+\frac{2}{K})e^{-4\log K} \notag\\
& \geq \frac{1}{K} - 3e^{-4\log K} \notag\\
& = \frac{1}{K} - 3(\frac{1}{K})^{4} \notag\\
& = \frac{1}{2K}
\end{align}
which is a contradiction.
\end{proof}

We then state the core lemmas of proving Lemma \ref{gmm_ti}. 

\begin{lemma} \label{lowerbound}
If for any i, $\|u_i-u_i^{*}\| \leq 16\sqrt{d \log K}$, then for $\Omega_{1}^{*}$ (corresponding results hold for each $\Omega_{i}^{*}$),
\%
\int_{\Omega_{1}^{*}}|P_{1}^{*}-P_{1}| \mathrm{d}x \geq c_{1} \min \left\{ \|u_{1}^{*}-u_{1}\|, 1 \right\},
\% where $c_{1}= \frac{1}{200}$.
\end{lemma}

\begin{lemma} \label{upperbound}
If for any i, $\|u_i-u_i^{*}\| \leq 16\sqrt{d \log K}$, then for $\Omega_{1}^{*}$ (corresponding results hold for each $\Omega_{i}^{*}$), then for every $j \neq 1$, 
\%
\int_{\Omega_{1}^{*}}|P_{j}^{*}-P_{j}| \mathrm{d}x \leq \frac{c_{2}}{K} \min \left\{ \|u_{j}^{*}-u_{j}\|, 1 \right\},
\% where $c_{2}= 2688 \left(\frac{1}{2}\right)^{69}.  $

\end{lemma}

With these lemmas, we are now able to prove Lemma \ref{gmm_ti}.
\begin{proof}[Proof of Lemma \ref{gmm_ti}]
By Lemma \ref{initial_match}, there exists a permutation of $\boldsymbol{u}$ such that $\|u_{i}^{*}-u_{i}\| \leq 16\sqrt{d\log{K}}$ holds for every $1\leq i \leq K$. Therefore Lemma \ref{lowerbound}, \ref{upperbound} can be applied. Notice that
\begin{align}
\int_{\Omega_{1}^{*}} |p_{\mathbf{u}}(x)- p_{\mathbf{u}^* }(x)| \mathrm{d}x 
&= \int_{\Omega_{1}^{*}} \bigg|\frac{1}{K}\sum_{i=1}^{K} P_{i}^{*}- \frac{1}{K}\sum_{i=1}^{K} P_{i}  \bigg| \mathrm{d}x \notag \\
& \geq \int_{\Omega_{1}^{*}} \bigg|\frac{1}{K} P_{1}^{*}- \frac{1}{K} P_{i}  \bigg| \mathrm{d}x -\int_{\Omega_{1}^{*}} \bigg|\frac{1}{K}\sum_{i=2}^{K} P_{i}^{*}- \frac{1}{K}\sum_{i=2}^{K} P_{i}  \bigg| \mathrm{d}x \notag \\
& \geq \frac{1}{K} \int_{\Omega_{1}^{*}} | P_{1}^{*}-  P_{i}  | \mathrm{d}x -\frac{1}{K}\sum_{i=2}^{K} \int_{\Omega_{1}^{*}} | P_{i}^{*}- P_{i}  | \mathrm{d}x \notag\\
& \geq \frac{c_{1}}{K} \min \left\{ \|u_{1}^{*}-u_{1}\|, 1 \right\} - \frac{c_{2}}{K^{2}} \sum_{i=2}^{K} \min \left\{ \|u_{i}^{*}-u_{i}\|, 1 \right\},
\end{align}
where the last line comes from Lemma \ref{lowerbound}, \ref{upperbound}. \\

Sum up all the equations above for corresponding $1 \leq i \leq K$, since $\{\Omega_{i}^{*}\}_{i=1}^{K}$ are disjoint, we have
\begin{align}
d_{\mathrm{TV}}\left(p_{\mathbf{u}}(x), p_{\mathbf{u}^* }(x)\right) &= \frac{1}{2} \int_{\R^{d}} |p_{\mathbf{u}}(x)- p_{\mathbf{u}^* }(x)| \mathrm{d}x \notag\\
&\geq \frac{1}{2}\sum_{i=1}^{K} \int_{\Omega_{i}^{*}} |p_{\mathbf{u}}(x)- p_{\mathbf{u}^* }(x)| \mathrm{d}x \notag \\
&\geq \frac{1}{2}\left( \frac{c_1}{K}- \frac{(K-1)c_{2}}{K^{2}} \right) \sum_{i=1}^{K} \min \left\{ \|u_{i}^{*}-u_{i}\|, 1 \right\} \notag \\
&\geq \frac{1}{2} \left( c_{1}- c_{2} \right) \cdot \frac{1}{K} \sum_{i=1}^{K} \min \left\{ \|u_{i}^{*}-u_{i}\|, 1 \right\} \notag \\
&=\frac{1}{2}\left(\frac{1}{200} - 2688 \left(\frac{1}{2}\right)^{69}\right) \cdot \frac{1}{K} \sum_{i=1}^{K} \min \left\{ \|u_{i}^{*}-u_{i}\|, 1 \right\} \notag \\
&\geq \frac{1}{500} \cdot \frac{1}{K} \sum_{i=1}^{K} \min \left\{ \|u_{i}^{*}-u_{i}\|, 1 \right\}.
\end{align}
In the end, we refer to Lemma \ref{tv_norm}, which states that 
\%
d_{\mathrm{TV}}(\mathcal{N}(u_{i}^{*}, I_{d}), \mathcal{N}(u_{i}, I_{d})) \leq \min ( \|u_{i}^{*}-u_{i}\|, 1).
\%
Take $\sigma(\boldsymbol{u})= \left\{u_i\right\}_{i=1}^K$,
\begin{align}
d_{\mathrm{TV}}\left(p_{\sigma(\mathbf{u})}(x, z), p_{\mathbf{u}^* }(x, z)\right) &= \sum_{i=1}^{K} \P (z=i) d_{\mathrm{TV}} (\mathcal{N}(u_{i}^{*},I_{d}),\mathcal{N}(u_{i},I_{d})) \notag \\
&\leq  \sum_{i=1}^{K} \frac{1}{K} \min ( \|u_{i}^{*}-u_{i}\|, 1) \notag \\
&\leq 500 d_{\mathrm{TV}}\left(p_{\mathbf{u}}(x), p_{\mathbf{u}^* }(x)\right).
\end{align}
\end{proof}
Finally we state the proof of Lemma \ref{lowerbound} and \ref{upperbound}. 

\begin{proof}[Proof of Lemma \ref{lowerbound}]
W.L.O.G.,let $u_{1}^{*}=0$, $\Delta:=\|u_{1}\| \leq 16\sqrt{d \log K}$, and $u_{1}=(-\Delta, 0, 0, \cdots, 0)$. The densities are given by
\%
P_{1}^{*}(x)=(\frac{1}{\sqrt{2\pi}})^{d} e^{-\frac{1}{2}\|x\|^{2}}
\%
\%
P_{1}(x)=(\frac{1}{\sqrt{2\pi}})^{d} e^{-\frac{1}{2}\|x-u_{1}\|^{2}}
\%
We consider an area $S \subset \Omega_{1}^{*}$:
\%
S:=\left\{ x=(x_{1},\cdots,x_{d}) \bigg| x \in \Omega_{1}^{*}, x_{1} \geq \frac{1}{10} \right\}
\%
Then for any $x \in S$, $\|x\|^{2} \leq \|x-u_{1}\|^{2}$, which implies $P_{1}^{*}(x) \geq P_{1}(x)$. Therefore
\begin{align}
\int_{\Omega_{1}^{*}} |P_{1}^{*}-P_{1}| \mathrm{d}x &\geq \int_{S}|P_{1}^{*}-P_{1}| \mathrm{d}x \notag \\
&= \int_{S} (\frac{1}{\sqrt{2\pi}})^{d} \left(e^{-\frac{1}{2}\|x\|^{2}} - e^{-\frac{1}{2}\|x-u_{1}\|^{2}} \right)\mathrm{d}x \notag\\
&=\int_{S} (\frac{1}{\sqrt{2\pi}})^{d} e^{-\frac{1}{2}\|x\|^{2}} \left(1- e^{\frac{1}{2}\|x\|^{2}-\frac{1}{2}\|x-u_{1}\|^{2}} \right) \mathrm{d}x \notag\\
&\geq \min_{x \in S} \left(1- e^{\frac{1}{2}\|x\|^{2}-\frac{1}{2}\|x-u_{1}\|^{2}} \right) \int_{S} (\frac{1}{\sqrt{2\pi}})^{d} e^{-\frac{1}{2}\|x\|^{2}} \mathrm{d}x \notag\\
&= \min_{x \in S} \left(1- e^{\frac{1}{2}\|x\|^{2}-\frac{1}{2}\|x-u_{1}\|^{2}} \right) \P(\mathcal{N}\left(0, I_d\right)\in S) 
\end{align}
For $\min_{x \in S} \left(1- e^{\frac{1}{2}\|x\|^{2}-\frac{1}{2}\|x-u_{1}\|^{2}} \right)$, notice that for any $x=(x_{1},\cdots,x_{d}) \in S$, 
\%
\frac{1}{2}\|x\|^{2}-\frac{1}{2}\|x-u_{1}\|^{2}=-x_1 \Delta - \frac{1}{2}\Delta^{2} \leq -\frac{1}{10}\Delta
\%
Thus 
\%
\min_{x \in S} \left(1- e^{\frac{1}{2}\|x\|^{2}-\frac{1}{2}\|x-u_{1}\|^{2}} \right) \geq 1-e^{-\frac{1}{10}\Delta}
\%
Take $c_{3}= \frac{1}{20}$. We claim that 
\%
\min_{x \in S} \left(1- e^{\frac{1}{2}\|x\|^{2}-\frac{1}{2}\|x-u_{1}\|^{2}} \right) \geq c_{3} \min\{\Delta,1\}.
\%
In fact, when $0 \leq \Delta \leq 1$,
\%
\min_{x \in S} \left(1- e^{\frac{1}{2}\|x\|^{2}-\frac{1}{2}\|x-u_{1}\|^{2}} \right) \geq 1-e^{-\frac{1}{10}\Delta} \geq \frac{1}{20} \Delta.
\%
The last inequality holds, since if we let $f(x)=e^{-\frac{1}{10}x}+\frac{1}{20}x-1$, Then $f(0)=0$,
\%
f'(x)=-\frac{1}{10}e^{-\frac{1}{10}x}+\frac{1}{20} \leq 0
\%
for any $x \in [0,10\log 2].$ Thus for any $\Delta\in [0,1]$, 
\%
e^{-\frac{1}{10}\Delta}+\frac{1}{20}\Delta-1 = f(\Delta) \leq f(0)=0.
\%
When $1\leq \Delta \leq 16\sqrt{d \log K}$, 
\%
\min_{x \in S} \left(1- e^{\frac{1}{2}\|x\|^{2}-\frac{1}{2}\|x-u_{1}\|^{2}} \right) \geq 1-e^{-\frac{1}{10}\Delta} \geq 1-e^{-\frac{1}{10}} \geq \frac{1}{20} \cdot 1
\%
Therefore we have shown that \%
\min_{x \in S} \left(1- e^{\frac{1}{2}\|x\|^{2}-\frac{1}{2}\|x-u_{1}\|^{2}} \right) \geq c_{3} \min\{\Delta,1\}.
\%
where $c_{3}=\frac{1}{20}$.\\\\
As for $\P(\mathcal{N}\left(0, I_d\right)\in S)$, take 
\%
S':=\left\{ x=(x_{1},\cdots,x_{d}) \bigg| 2\sqrt{d\log2} \geq x_{1} \geq \frac{1}{10}, x_{2}^{2}+ \cdots + x_{d}^{2} \leq 60d \log K \right\}.
\%
Then $S' \subset S$. Therefore 
\begin{align}
\P(\mathcal{N}\left(0, I_d\right)\in S) &\geq \P(\mathcal{N}\left(0, I_d\right)\in S') \notag \\
&= \P(2\sqrt{d\log2} \geq x_{1} \geq \frac{1}{10},x_{2}^{2}+ \cdots + x_{d}^{2} \leq 60d \log K,x \sim \mathcal{N}\left(0, I_d\right))\notag \\
&=\P\left(2\sqrt{d\log2} \geq \mathcal{N}(0, 1)\geq \frac{1}{10}\right) \P\left(\left\|\mathcal{N}(0, I_{d-1})\right\|^{2} \leq 60d \log K\right) \notag \\
& \geq  \P\left(2\sqrt{\log2} \geq \mathcal{N}(0, 1)\geq \frac{1}{10}\right) \P\left(\left\|\mathcal{N}(0, I_{d-1})\right\|^{2} \leq 60(d-1) \log 2\right) \notag \\
& > \P\left(2\sqrt{\log2} \geq \mathcal{N}(0, 1)\geq \frac{1}{10}\right) \cdot (1-2e^{-2}) \quad \text{(by Lemma \ref{norm_subGaussian})}\notag \\
& > \frac{1}{4} \cdot (1-2e^{-2}) \quad \notag \\
&> \frac{1}{10}
\end{align}
Combine all these results, we have
\begin{align}
\int_{\Omega_{1}^{*}} |P_{1}^{*}-P_{1}| \mathrm{d}x  &\geq \min_{x \in S} \left(1- e^{\frac{1}{2}\|x\|^{2}-\frac{1}{2}\|x-u_{1}\|^{2}} \right) \P(\mathcal{N}\left(0, I_d\right)\in S) \notag \\
&\geq c_{3} \min\{\Delta,1\} \cdot \frac{1}{10} \notag\\
&=\frac{1}{200} \min\{\|u_{1}^{*}-u_{1}\|,1\} 
\end{align}
\end{proof}


\begin{proof}[Proof of Lemma \ref{upperbound}]
For any $i \neq 1$, 
\%
\int_{\Omega_{1}^{*}} |P_{i}^{*}-P_{i}| \mathrm{d}x = \int_{\Omega_{1}^{*}} (\frac{1}{\sqrt{2\pi}})^{d} | e^{-\frac{1}{2}\|x-u_{i}^{*}\|^{2}} - e^{-\frac{1}{2}\|x-u_{i}\|^{2}}  | \mathrm{d}x.
\%
Notice that if we denote $a(x):= \|x-u_{i}^{*}\|$, $\delta(x):= \|x-u_{i}^{*}\|- \|x-u_{i}\|$ ,$\Delta:=\|u_{i}-u_{i}^{*}\|$, then $|\delta(x)| \leq \Delta \leq 16\sqrt{d\log K}$, and for any $x\in \Omega_{1}^{*}$, $a(x) \geq 92\sqrt{d \log K}$ (due to separation condition). Therefore
\begin{align}
& \max_{x \in \Omega_{1}^{*}} \bigg| e^{-\frac{1}{2}\|x-u_{i}^{*}\|^{2}} - e^{-\frac{1}{2}\|x-u_{i}\|^{2}}  \bigg| \notag\\
&= \max_{x \in \Omega_{1}^{*}} \bigg| e^{-\frac{1}{2}a(x)^{2}} -  e^{-\frac{1}{2}(a(x)-\delta (x))^{2}} \bigg| \notag\\
& \leq \max \left\{ \bigg| e^{-\frac{1}{2}a(x)^{2}} -  e^{-\frac{1}{2}(a(x)-\delta (x))^{2}} \bigg| \Bigg| a(x) \geq 92\sqrt{d \log K}, |\delta(x)| \leq \Delta   \right\} \notag\\
&\leq \max_{a \geq 92\sqrt{d \log K}} \{ \max ( |e^{-\frac{a^{2}}{2}}- e^{-\frac{(a-\Delta)^{2}}{2}}| , |e^{-\frac{a^{2}}{2}}- e^{-\frac{(a+\Delta)^{2}}{2}}|) \} \notag\\
&= \max_{a \geq 92\sqrt{d \log K}} \{ \max ( e^{-\frac{(a-\Delta)^{2}}{2}} - e^{-\frac{a^{2}}{2}} , e^{-\frac{a^{2}}{2}}- e^{-\frac{(a+\Delta)^{2}}{2}}) \} \notag\\
& \leq \max (\max_{a \geq 92\sqrt{d \log K}} e^{-\frac{(a-\Delta)^{2}}{2}} - e^{-\frac{a^{2}}{2}}, \max_{a \geq 92\sqrt{d \log K}} e^{-\frac{a^{2}}{2}}- e^{-\frac{(a+\Delta)^{2}}{2}})) \notag\\
& \leq \max (\max_{a \geq 76\sqrt{d \log K}} e^{-\frac{a^{2}}{2}}- e^{-\frac{(a+\Delta)^{2}}{2}}, \max_{a \geq 92\sqrt{d \log K}} e^{-\frac{a^{2}}{2}}- e^{-\frac{(a+\Delta)^{2}}{2}})) .
\end{align}
The last inequality holds since $\Delta \leq 16\sqrt{d\log K}$. For fixed $\Delta$, let $f(a)=e^{-\frac{a^{2}}{2}}- e^{-\frac{(a+\Delta)^{2}}{2}}$. Then 
\%
f'(a)=-a e^{-\frac{a^{2}}{2}} + (a+\Delta)e^{-\frac{(a+\Delta)^{2}}{2}}
\%
We first show that $f'(a) \leq 0$, for any $a\geq 76\sqrt{d\log K}$.
Notice that 
\begin{align}
f'(a) &=-a e^{-\frac{a^{2}}{2}} + (a+\Delta)e^{-\frac{(a+\Delta)^{2}}{2}} \leq 0 \notag\\
& \iff (a+\Delta)e^{-\frac{(a+\Delta)^{2}}{2}} \leq a e^{-\frac{a^{2}}{2}} \notag\\
& \iff 1+ \frac{\Delta}{a} \leq e^{a\Delta + \frac{1}{2}\Delta^{2}}
\end{align}
The last statement is true because 
\%
e^{a\Delta + \frac{1}{2}\Delta^{2}} \geq 1 + a\Delta + \frac{1}{2}\Delta^{2} \geq 1+ \frac{\Delta}{a}
\%
when $a\geq 76\sqrt{d\log K} > 1.$ \\
Since $f'(a) \leq 0$ for any $a\geq 76\sqrt{d\log K}$, we have
\begin{align}
f(a) &\leq f(76\sqrt{d \log{K}}) \notag\\
&= \exp (-\frac{1}{2} (76\sqrt{d \log{K}})^{2}) - \exp (-\frac{1}{2} (76\sqrt{d \log{K}} + \Delta )^{2})\notag\\
&= e^{-\frac{1}{2} (76\sqrt{d \log{K}})^{2}} (1- e^{-76\sqrt{d \log K} \Delta -\frac{1}{2}\Delta^{2} } ) \notag\\
&\leq e^{-\frac{1}{2} (76\sqrt{d \log{K}})^{2}} (76\sqrt{d \log K} \Delta +\frac{1}{2}\Delta^{2}) \notag\\
&\leq e^{-\frac{1}{2} (76\sqrt{d \log{K}})^{2}} \cdot 84\sqrt{d \log K} \Delta \quad \text{(since $\Delta \leq 16 \sqrt{d \log K}$)}.
\end{align}
Which shows 
\%
\max_{a \geq 76\sqrt{d \log K}} e^{-\frac{a^{2}}{2}}- e^{-\frac{(a+\Delta)^{2}}{2}} \leq e^{-\frac{1}{2} (76\sqrt{d \log{K}})^{2}} \cdot 84\sqrt{d \log K} \Delta
\%
Similarly
\%
\max_{a \geq 92\sqrt{d \log K}} e^{-\frac{a^{2}}{2}}- e^{-\frac{(a+\Delta)^{2}}{2}} \leq e^{-\frac{1}{2} (92\sqrt{d \log{K}})^{2}} \cdot 100\sqrt{d \log K} \Delta
\%
Therefore 
\%
\max_{x \in \Omega_{1}^{*}} \bigg| e^{-\frac{1}{2}\|x-u_{i}^{*}\|^{2}} - e^{-\frac{1}{2}\|x-u_{i}\|^{2}}  \bigg| \leq e^{-\frac{1}{2} (76\sqrt{d \log{K}})^{2}} \cdot 84\sqrt{d \log K} \Delta \leq c_4 \min \left\{ \|u_{i}^{*}-u_{i}\|, 1 \right\}
\% 
where $c_4=e^{-\frac{1}{2} (76\sqrt{d \log{K}})^{2}} \cdot 1344 d \log K$ (Since $\Delta \leq 16\sqrt{d \log K} \min \left\{ \Delta, 1 \right\}$).
Notice that 
\begin{align}
c_{4} &= e^{-\frac{1}{2} (76\sqrt{d \log{K}})^{2}} \cdot 1344 d \log K \notag \\
&\leq e^{-\frac{1}{2} (76\sqrt{d \log{K}})^{2}} \cdot 1344 k^{d} K \notag\\
&\leq e^{-\frac{1}{2} (76\sqrt{d \log{K}})^{2}} \cdot 1344 k^{2d}
\notag\\
&= 1344 e^{-2886d \log K} \notag \\
& \leq 1344 e ^{-\frac{1}{2} (70\sqrt{d \log{K}})^{2}}
\end{align}
W.L.O.G., let $u_{1}^{*}=0$, and define $ u'= (50\sqrt{d \log K},0, \cdots, 0)$, then 

\begin{align}
\int_{\Omega_{1}^{*}} |P_{i}^{*}-P_{i}| \mathrm{d}x &= \int_{\Omega_{1}^{*}} (\frac{1}{\sqrt{2\pi}})^{d} | e^{-\frac{1}{2}\|x-u_{i}^{*}\|^{2}} - e^{-\frac{1}{2}\|x-u_{i}\|^{2}}  | \mathrm{d}x \notag\\
&\leq \int_{\Omega_{1}^{*}} (\frac{1}{\sqrt{2\pi}})^{d} \max_{x\in \Omega_{1}^{*}} | e^{-\frac{1}{2}\|x-u_{i}^{*}\|^{2}} - e^{-\frac{1}{2}\|x-u_{i}\|^{2}}  | \mathrm{d}x \notag\\
&\leq \int_{\Omega_{1}^{*}} (\frac{1}{\sqrt{2\pi}})^{d} 1344 e ^{-\frac{1}{2} (70\sqrt{d \log{K}})^{2}} \min \left\{ \|u_{i}^{*}-u_{i}\|, 1 \right\} \mathrm{d}x\notag\\
& = \min \left\{ \|u_{i}^{*}-u_{i}\|, 1 \right\} \int_{\Omega_{1}^{*}} (\frac{1}{\sqrt{2\pi}})^{d} 1344 e ^{-\frac{1}{2} (70\sqrt{d \log{K}})^{2}}  \mathrm{d}x \notag\\
& \leq 1344 \min \left\{ \|u_{i}^{*}-u_{i}\|, 1 \right\} \int_{\Omega_{1}^{*}} (\frac{1}{\sqrt{2\pi}})^{d} e^{-\frac{1}{2}\|x-u'\|^{2}}\mathrm{d}x \notag\\
& \leq 1344 \min \left\{ \|u_{i}^{*}-u_{i}\|, 1 \right\} \P (\mathcal{N}\left(u', I_d\right)\in \Omega_{1}^{*}) \notag\\
& \leq 1344 \min \left\{ \|u_{i}^{*}-u_{i}\|, 1 \right\} \P (\|\mathcal{N}\left(u', I_d\right)-u'\| \geq 34\sqrt{d \log K}) \notag\\
& \leq 1344 \min \left\{ \|u_{i}^{*}-u_{i}\|, 1 \right\} \cdot 2\exp(-\frac{(34\sqrt{d \log K})^{2}}{16d})\quad\text{(by Lemma \ref{norm_subGaussian})} \notag\\
&\leq 1344 \min \left\{ \|u_{i}^{*}-u_{i}\|, 1 \right\} \cdot 2\exp(-70\log K)\notag\\
&= 2688 \min \left\{ \|u_{i}^{*}-u_{i}\|, 1 \right\} \left(\frac{1}{K}\right)^{70} \notag\\
&\leq 2688 \left(\frac{1}{2}\right)^{69} \left(\frac{1}{K}\right) \min \left\{ \|u_{i}^{*}-u_{i}\|, 1 \right\}
\end{align}

\end{proof}