\section{Proof of Proposition~\ref{prop:distanceinequalities}}
\label{sec:distanceinequalities}
Recall that we will prove this for restrictions of probability distributions to subsets of the support -- in other words, we do not assume $\sum_{i \in S} p_i = \sum_{i \in S} q_i = 1$, we only assume that $\sum_{i \in S} p_i \leq 1$ and $\sum_{i \in S} q_i \leq 1$.
\paragraph{$\dh^2(p_S,q_S) \leq \dtv(p_S,q_S):$}
\begin{align*}
\dh^2(p_S,q_S) &= \frac12 \sum_{i \in S} (\sqrt{p_i} - \sqrt{q_i})^2 \\
&\leq \frac12 \sum_{i \in S} |\sqrt{p_i} - \sqrt{q_i}|(\sqrt{p_i} + \sqrt{q_i}) \\
&= \frac12 \sum_{i \in S} |p_i - q_i| \\
&= \dtv(p_S,q_S).
\end{align*}

\paragraph{$\dtv(p_S,q_S) \leq \sqrt{2}\dh(p_S,q_S):$}
\begin{align*}
\dtv^2(p_S,q_S) &= \frac14 \left(\sum_{i \in S} \left|p_i - q_i\right|\right)^2 \\
&= \frac14 \left(\sum_{i \in S} \left|\sqrt{p_i} -\sqrt{q_i}\right|(\sqrt{p_i} + \sqrt{q_i})\right)^2 \\
&\leq \frac14 \left(\sum_{i \in S} \left|\sqrt{p_i} -\sqrt{q_i}\right|^2\right)\left(\sum_{i \in S}(\sqrt{p_i} + \sqrt{q_i})^2\right) \\
&\leq \dh^2(p_S, q_S) \cdot \frac12 \left(\sum_{i \in S}(\sqrt{p_i} + \sqrt{q_i})^2\right) \\
&= \dh^2(p_S, q_S) \cdot \left(\sum_{i \in S}p_i + \sum_{i \in S} q_i - \dh^2(p_S,q_S)\right) \\
&\leq \dh^2(p_S,q_S) \cdot \left(2 - \dh^2(p_S,q_S)\right) \\
&\leq 2 \dh^2(p_S,q_S).
\end{align*}
Taking the square root of both sides gives the result.
The second inequality is Cauchy-Schwarz.

\paragraph{$2\dh^2(p_S, q_S) \leq \sum_{i \in S} (q_i - p_i) + \dkl(p_S, q_S):$}
\begin{align*}
2 \dh^2(p_S, q_S) 
&= \sum_{i \in S} (q_i + p_i) - 2\sum_{i \in S} \sqrt{p_i q_i} \\
&= \sum_{i \in S} (q_i + p_i) - 2\left(\left(\sum_{j \in S} p_j\right)\sum_{i \in S} \frac{p_i}{\sum_{j \in S} p_j} \sqrt{\frac{q_i}{p_i}}\right) \\
&\leq \sum_{i \in S} (q_i + p_i) - 2\left(\left(\sum_{j \in S} p_j\right)\exp\left(\frac12 \sum_{i \in S} \frac{p_i}{\sum_{j \in S} p_j} \log{\frac{q_i}{p_i}}\right)\right) \\
&\leq \sum_{i \in S} (q_i + p_i) - 2\left(\left(\sum_{j \in S} p_j\right)\left(1 + \frac12 \sum_{i \in S} \frac{p_i}{\sum_{j \in S} p_j} \log{\frac{q_i}{p_i}}\right)\right) \\
&= \sum_{i \in S} (q_i - p_i) - \left(\sum_{i \in S} p_i \log{\frac{q_i}{p_i}} \right)\\
&= \sum_{i \in S} (q_i - p_i) + \dkl(p_S, q_S).
\end{align*}
The first inequality is Jensen's, and the second is $1 + x \leq \exp(x)$.

\paragraph{$\dkl(p_S, q_S) \leq \sum_{i \in S} (p_i - q_i) +  \dxs(p_S, q_S):$}
\begin{align*}
\dkl(p_S, q_S) 
&= \left(\sum_{j \in S} p_j\right)\left(\sum_{i \in S} \frac{p_i}{\sum_{j \in S} p_j} \log{\frac{p_i}{q_i}}\right) \\
&\leq \left(\sum_{j \in S} p_j\right)\left(\log {\frac{1}{\sum_{j\in S} p_j}\sum_{i \in S} \frac{p_i^2}{q_i}} \right) \\
&= \left(\sum_{j \in S} p_j\right) \left(\log{ \left(\frac{1}{\sum_{j\in S} p_j} \left(\dxs(p_S, q_S) + 2\sum_{i \in S} p_i - \sum_{i \in S} q_i\right)\right)} \right) \\
&= \left(\sum_{j \in S} p_j\right) \left(\log{  \left(2 + \frac{1}{\sum_{j\in S} p_j} \left(\dxs(p_S, q_S)  - \sum_{i \in S} q_i\right)\right)} \right) \\
&\leq \left(\sum_{j \in S} p_j\right) \left(1 + \frac{1}{\sum_{j\in S} p_j} \left(\dxs(p_S, q_S)  - \sum_{i \in S} q_i\right)\right) \\
&=\sum_{i \in S} (p_i - q_i) +  \dxs(p_S, q_S).
\end{align*}
The first inequality is Jensen's, and the second is $1 + x \leq \exp(x)$.
